A checker whether a certain object was visited or not is not needed anymore.

src/Ex/MsiSvInv.v
@@ -14,6 +14,115 @@ Open Scope list.
 Open Scope hvec.
 Open Scope fmap.
 
+Ltac disc_AtomicInv :=
+  repeat
+    match goal with
+    | [H: AtomicInv _ _ _ _ _ _ |- _] => red in H; dest
+    end.
+
+Ltac atomic_cont_exfalso_bound msgOutPred :=
+  exfalso;
+  disc_rule_conds_ex;
+  repeat 
+    match goal with
+    | [H1: AtomicMsgOutsInv _ ?eouts _, H2: In _ ?eouts |- _] =>
+      red in H1; rewrite Forall_forall in H1;
+      specialize (H1 _ H2); simpl in H1
+    | [H: msgOutPred _ _ _ |- _] => red in H
+    | [H1: caseDec _ ?sig _ _ |- _] =>
+      match sig with
+      | sigOf (?midx, ?msg) =>
+        match goal with
+        | [H2: msg_id ?msg = ?mid, H3: msg_type ?msg = ?mty |- _] =>
+          progress replace sig with (midx, (mty, mid)) in H1
+            by (unfold sigOf; simpl; rewrite H2, H3; reflexivity);
+          simpl in H1
+        end
+      end
+    end;
+  assumption.
+
+Ltac atomic_init_exfalso_rq :=
+  exfalso;
+  disc_rule_conds_ex;
+  repeat
+    match goal with
+    | [H: _ = _ \/ _ |- _] =>
+      destruct H; [subst; try discriminate|auto]
+    end.
+
+Ltac atomic_init_exfalso_rs_from_parent :=
+  exfalso;
+  repeat
+    (repeat match goal with
+            | [H: UpLockInvORq _ _ _ _ _ |- _] => red in H
+            | [H1: ?orq@[0] = Some _, H2: context[?orq@[0]] |- _] =>
+              rewrite H1 in H2; simpl in H2
+            | [H: UpLockRsFromParent _ _ _ |- _] =>
+              let rsFrom := fresh "rsFrom" in
+              destruct H as [rsFrom [? ?]]
+            end;
+     disc_rule_conds_ex);
+  repeat
+    match goal with
+    | [H1: _ = ?rsFrom \/ _, H2: edgeDownTo _ _ = Some ?rsFrom |- _] =>
+      destruct H1; [subst; try discriminate|auto]
+    end.
+
+Ltac atomic_init_solve_AtomicMsgOutsInv :=
+  simpl; repeat constructor.
+
+(* Ltac atomic_init_solve_AtomicLocksInv := *)
+(*   red; intros; dest_in; *)
+(*   repeat (simpl; mred); *)
+(*   unfold sigOf; simpl; *)
+(*   repeat *)
+(*     match goal with *)
+(*     | [H: msg_id ?msg = _ |- context [msg_id ?msg] ] => rewrite H *)
+(*     | [H1: msg_id ?msg = _, H2: context [msg_id ?msg] |- _] => *)
+(*       rewrite H1 in H2 *)
+(*     | [H: ?orq@[?i] = Some _ |- context [?orq@[?i]] ] => rewrite H *)
+(*     | [H1: ?orq@[?i] = Some _, H2: context [?orq@[?i]] |- _] => *)
+(*       rewrite H1 in H2 *)
+(*     | [H: ?orq@[?i] = None |- context [?orq@[?i]] ] => rewrite H *)
+(*     | [H1: ?orq@[?i] = None, H2: context [?orq@[?i]] |- _] => *)
+(*       rewrite H1 in H2 *)
+(*     end; *)
+(*   repeat (red; simpl; mred; auto). *)
+
+Ltac atomic_init_solve_AtomicInv :=
+  atomic_init_solve_AtomicMsgOutsInv.
+
+Ltac disc_sig_caseDec :=
+  match goal with
+  | [H1: caseDec _ ?sig _ _ |- _] =>
+    match sig with
+    | sigOf (?midx, ?msg) =>
+      match goal with
+      | [H2: msg_id ?msg = ?mid, H3: msg_type ?msg = ?mty |- _] =>
+        progress replace sig with (midx, (mty, mid)) in H1
+          by (unfold sigOf; simpl; rewrite H2, H3; reflexivity);
+        simpl in H1
+      end
+    end
+  end.
+
+Ltac disc_msg_preds_with Hl Hin :=
+  match type of Hl with
+  | AtomicMsgOutsInv _ ?eouts _ =>
+    red in Hl; rewrite Forall_forall in Hl;
+    specialize (Hl _ Hin); simpl in Hl;
+    red in Hl; disc_sig_caseDec
+  end.
+
+Ltac disc_msg_preds Hin :=
+  match goal with
+  | [H: AtomicMsgOutsInv _ _ _ |- _] =>
+    let Hl := fresh "H" in
+    pose proof H as Hl;
+    disc_msg_preds_with Hl Hin
+  end.
+
 Section Inv.
 
   (** Basic predicates per an object *)
@@ -44,7 +153,7 @@ Section Inv.
 
   Section GInv.
     Variables (post cost1 cost2: OState ImplOStateIfc)
-              (corq1 corq2: ORq Msg).
+              (porq corq1 corq2: ORq Msg).
 
     (** The first invariant: the directory status is coherent to statuses of
      * children. Note that an object is *not* required to keep the coherency
@@ -81,6 +190,11 @@ Section Inv.
       ImplChildCoh1 cv /\ ImplChildCoh2 cv /\
       ImplChildrenCoh.
 
+    Definition ImplParentLockInv: Prop :=
+      rqid <+- porq@[downRq];
+        ((rqid.(rqi_minds_rss) = [c2pRs] /\ rqid.(rqi_midx_rsb) = pc1) \/
+         (rqid.(rqi_minds_rss) = [c1pRs] /\ rqid.(rqi_midx_rsb) = pc2)).
+    
   End GInv.
 
   Definition ImplStateInv (st: MState ImplOStateIfc): Prop :=
@@ -90,7 +204,14 @@ Section Inv.
       corq1 <-- (bst_orqs st)@[child1Idx];
       corq2 <-- (bst_orqs st)@[child2Idx];
       (exists cv, ImplStateCoh post cost1 cost2 corq1 corq2 cv) /\
-      (ImplDirCoh post cost1 cost2 corq1 corq2).
+      ImplDirCoh post cost1 cost2 corq1 corq2.
+
+  Definition ImplLockInv (st: MState ImplOStateIfc): Prop :=
+    porq <-- (bst_orqs st)@[parentIdx];
+      ImplParentLockInv porq.
+
+  Definition ImplInv (st: MState ImplOStateIfc): Prop :=
+    ImplStateInv st /\ ImplLockInv st.
 
   Hint Unfold ImplOStateM ImplOStateS ImplOStateI ImplOStateMSI
        ImplDirM ImplDirS ImplDirI
@@ -153,24 +274,30 @@ Section Inv.
       mred.
     Qed.
 
-    Lemma implStateInv_orqs_weakened:
+    Lemma implInv_orqs_weakened:
       forall st oidx orq norq rqt rqi nmsgs,
-        ImplStateInv st ->
+        ImplInv st ->
+        (oidx = child1Idx \/ oidx = child2Idx) ->
         (bst_orqs st)@[oidx] = Some orq ->
         norq = orq +[rqt <- rqi] ->
-        ImplStateInv {| bst_oss := bst_oss st;
-                        bst_orqs := (bst_orqs st) +[oidx <- norq];
-                        bst_msgs := nmsgs |}.
+        ImplInv {| bst_oss := bst_oss st;
+                   bst_orqs := (bst_orqs st) +[oidx <- norq];
+                   bst_msgs := nmsgs |}.
     Proof.
-      unfold ImplStateInv; simpl; intros.
-      disc_rule_conds_const.
-      destruct H as [[cv [? ?]] ?].
-      solve_rule_conds_ex.
+      unfold ImplInv, ImplStateInv, ImplLockInv; simpl; intros; dest.
+      split.
+      - disc_rule_conds_const.
+        destruct H as [[cv ?] ?].
+        destruct H0; subst.
+        + solve_rule_conds_ex.
+        + solve_rule_conds_ex.
+      - disc_rule_conds_const.
+        destruct H0; subst; mred.
     Qed.
 
-    Lemma implStateCoh_M_value_changed:
+    Lemma implInv_M_value_changed:
       forall st,
-        ImplStateInv st ->
+        ImplInv st ->
         forall oidx ost orq,
           (oidx = child1Idx \/ oidx = child2Idx) ->
           (bst_oss st)@[oidx] = Some ost ->
@@ -178,56 +305,60 @@ Section Inv.
           (bst_orqs st)@[oidx] = Some orq ->
           orq@[upRq] = None ->
           forall n (uv: DirT * unit) nmsgs,
-            ImplStateInv
+            ImplInv
               (Build_MState
                  (oifc:= ImplOStateIfc)
                  ((bst_oss st) +[oidx <- (n, (msiM, uv))])
                  (bst_orqs st) nmsgs).
     Proof.
-      unfold ImplStateInv; simpl; intros.
-      disc_rule_conds_const.
-      destruct H as [[cv ?] ?].
-      disc_rule_conds_ex.
-      - destruct H0; discriminate.
-      - split.
-        + exists n; repeat split.
-          * disc_rule_conds_ex.
-            destruct H as [|[|]];
-              try (exfalso; solve_rule_conds_ex; solve_msi; fail).
-            right; right.
-            solve_rule_conds_ex.
-          * solve_rule_conds_ex; solve_msi.
+      unfold ImplInv, ImplStateInv, ImplLockInv; simpl; intros; dest.
+      split.
+      - disc_rule_conds_const.
+        destruct H as [[cv ?] ?].
+        disc_rule_conds_ex.
+        + destruct H0; discriminate.
+        + split.
+          * exists n; repeat split.
+            { disc_rule_conds_ex.
+              destruct H as [|[|]];
+                try (exfalso; solve_rule_conds_ex; solve_msi; fail).
+              right; right.
+              solve_rule_conds_ex.
+            }
+            { solve_rule_conds_ex; solve_msi. }
+            { solve_rule_conds_ex. }
+            { solve_rule_conds_ex. }
           * solve_rule_conds_ex.
+        + split.
+          * exists n; repeat split.
+            { disc_rule_conds_ex.
+              destruct H as [|[|]];
+                try (exfalso; solve_rule_conds_ex; solve_msi; fail).
+              right; right.
+              solve_rule_conds_ex.
+            }
+            { solve_rule_conds_ex; solve_msi. }
+            { solve_rule_conds_ex. }
+            { solve_rule_conds_ex. }
           * solve_rule_conds_ex.
-        + solve_rule_conds_ex.
-      - split.
-        + exists n; repeat split.
-          * disc_rule_conds_ex.
-            destruct H as [|[|]];
-              try (exfalso; solve_rule_conds_ex; solve_msi; fail).
-            right; right.
-            solve_rule_conds_ex.
-          * solve_rule_conds_ex; solve_msi.
-          * solve_rule_conds_ex.
-          * solve_rule_conds_ex.
-        + solve_rule_conds_ex.
-      - eauto 7.
+        + eauto 7.
+      - assumption.
     Qed.
 
     Lemma msiSv_impl_InvTrs_ext_in:
       forall st1 eins st2,
-        ImplStateInv st1 ->
+        ImplInv st1 ->
         step_m impl st1 (RlblIns eins) st2 ->
-        ImplStateInv st2.
+        ImplInv st2.
     Proof.
       intros; inv_step; assumption.
     Qed.
 
     Lemma msiSv_impl_InvTrs_ext_out:
       forall st1 eouts st2,
-        ImplStateInv st1 ->
+        ImplInv st1 ->
         step_m impl st1 (RlblOuts eouts) st2 ->
-        ImplStateInv st2.
+        ImplInv st2.
     Proof.
       intros; inv_step; assumption.
     Qed.
@@ -400,40 +531,6 @@ Section Inv.
         auto.
     Qed.
 
-    Definition MsiSvLockPred (oidx: IdxT) (orq: ORq Msg): Prop :=
-      match case oidx on eq_nat_dec default True with
-      | child1Idx: True
-      | child2Idx: True
-      | parentIdx:
-          rqid <+- orq@[downRq];
-          ((rqid.(rqi_minds_rss) = [c2pRs] /\ rqid.(rqi_midx_rsb) = pc1) \/
-           (rqid.(rqi_minds_rss) = [c1pRs] /\ rqid.(rqi_midx_rsb) = pc2))
-      end.
-
-    Ltac obj_visited_rsDown oidx :=
-      try match goal with
-          | [Ha: Atomic _ _ _ ?hst _ _ |- _] =>
-            assert (In oidx (oindsOf hst))
-              by (eapply extAtomic_rsDown_acceptor_visited; eauto;
-                  [exact msiSv_impl_ORqsInit
-                  |exact msiSv_impl_RqRsSys
-                  |econstructor; eassumption
-                  |red; auto])
-          end.
-
-    Ltac obj_visited_rsUp oidx ocidx :=
-      try match goal with
-          | [Ha: Atomic _ _ _ ?hst _ _ |- _] =>
-            assert (In parentIdx (oindsOf hst))
-              by (eapply extAtomic_rsUp_acceptor_visited
-                    with (cidx:= ocidx); eauto;
-                  [exact msiSv_impl_ORqsInit
-                  |exact msiSv_impl_RqRsSys
-                  |econstructor; eassumption
-                  |red; auto
-                  |reflexivity])
-          end.
-    
     Ltac disc_rule_custom ::=
       try disc_footprints_ok;
       try disc_AtomicInv.
@@ -441,14 +538,14 @@ Section Inv.
     Lemma msiSv_impl_InvTrs_init:
       forall st1,
         Reachable (steps step_m) impl st1 ->
-        ImplStateInv st1 ->
+        ImplInv st1 ->
         forall oidx ridx ins outs st2,
           SubList (idsOf ins) (sys_merqs impl) ->
           step_m impl st1 (RlblInt oidx ridx ins outs) st2 ->
           AtomicInv
-            MsiSvMsgOutPred MsiSvLockPred
+            MsiSvMsgOutPred
             ins st1 [RlblInt oidx ridx ins outs] outs st2 /\
-          ImplStateInv st2.
+          ImplInv st2.
     Proof.
       intros.
       inv_step.
@@ -491,25 +588,25 @@ Section Inv.
         disc_rule_conds_ex.
         simpl; split; [atomic_init_solve_AtomicInv|].
         replace (oss +[child1Idx <- pos]) with oss by meq.
-        eapply implStateInv_orqs_weakened in H0; eauto.
+        eapply implInv_orqs_weakened in H0; eauto.
 
       - (** [childSetRqImm] *)
         disc_rule_conds_ex.
         simpl; split; [atomic_init_solve_AtomicInv|].
         replace (orqs +[child1Idx <- norq]) with orqs by meq.
-        eapply implStateCoh_M_value_changed in H0; eauto.
+        eapply implInv_M_value_changed in H0; eauto.
 
       - (** [childSetRqM] *)
         disc_rule_conds_ex.
         simpl; split; [atomic_init_solve_AtomicInv|].
         replace (oss +[child1Idx <- pos]) with oss by meq.
-        eapply implStateInv_orqs_weakened in H0; eauto.
+        eapply implInv_orqs_weakened in H0; eauto.
 
       - (** [childEvictRqI] *)
         disc_rule_conds_ex.
         simpl; split; [atomic_init_solve_AtomicInv|].
         replace (oss +[child1Idx <- pos]) with oss by meq.
-        eapply implStateInv_orqs_weakened in H0; eauto.
+        eapply implInv_orqs_weakened in H0; eauto.
 
       - (** [childGetRqImm] *)
         disc_rule_conds_ex.
@@ -522,25 +619,25 @@ Section Inv.
         disc_rule_conds_ex.
         simpl; split; [atomic_init_solve_AtomicInv|].
         replace (oss +[child2Idx <- pos]) with oss by meq.
-        eapply implStateInv_orqs_weakened in H0; eauto.
+        eapply implInv_orqs_weakened in H0; eauto.
 
       - (** [childSetRqImm] *)
         disc_rule_conds_ex.
         simpl; split; [atomic_init_solve_AtomicInv|].
         replace (orqs +[child2Idx <- norq]) with orqs by meq.
-        eapply implStateCoh_M_value_changed in H0; eauto.
+        eapply implInv_M_value_changed in H0; eauto.
 
       - (** [childSetRqM] *)
         disc_rule_conds_ex.
         simpl; split; [atomic_init_solve_AtomicInv|].
         replace (oss +[child2Idx <- pos]) with oss by meq.
-        eapply implStateInv_orqs_weakened in H0; eauto.
+        eapply implInv_orqs_weakened in H0; eauto.
 
       - (** [childEvictRqI] *)
         disc_rule_conds_ex.
         simpl; split; [atomic_init_solve_AtomicInv|].
         replace (oss +[child2Idx <- pos]) with oss by meq.
-        eapply implStateInv_orqs_weakened in H0; eauto.
+        eapply implInv_orqs_weakened in H0; eauto.
     Qed.
 
     Ltac disc_rule_custom ::=
@@ -550,13 +647,13 @@ Section Inv.
       try disc_msi;
       try disc_minds_const.
 
-    Lemma msiSv_impl_InvTrs: InvTrs impl ImplStateInv.
+    Lemma msiSv_impl_InvTrs: InvTrs impl ImplInv.
     Proof.
       eapply inv_atomic_InvTrs;
         [red; intros; eapply msiSv_impl_InvTrs_ext_in; eauto
         |red; intros; eapply msiSv_impl_InvTrs_ext_out; eauto
         |].
-      instantiate (1:= AtomicInv MsiSvMsgOutPred MsiSvLockPred).
+      instantiate (1:= AtomicInv MsiSvMsgOutPred).
       red; intros.
       destruct H1.
       generalize dependent ist2.
@@ -591,86 +688,74 @@ Section Inv.
         good_footprint_get child1Idx.
         disc_rule_conds_ex.
 
-        (* discharge lock predicates *)
-        obj_visited_rsDown child1Idx.
-        disc_lock_preds child1Idx.
-        disc_rule_conds_ex.
-
         (* discharge message predicates *)
         disc_msg_preds H4.
         disc_rule_conds_ex.
 
         (* generate hints for leaves (L1 caches) *)
-        pose proof (parentIdxOf_child_indsOf _ _ H8).
+        pose proof (parentIdxOf_child_indsOf _ _ H7).
         dest_in; try discriminate; simpl in *.
-        cbn in H27; inv H27.
+        cbn in H26; inv H26.
 
         (* construction *)
         split.
-        + split.
-          * apply Forall_app.
-            { apply forall_removeOnce.
-              eapply atomic_rsDown_preserves_msg_out_preds; eauto;
-                [exact msiSv_impl_ORqsInit
-                |exact msiSv_impl_RqRsSys
-                |red; auto
-                |exact msiSvMsgOutPred_good].
+        + apply Forall_app.
+          * apply forall_removeOnce.
+            eapply atomic_rsDown_preserves_msg_out_preds; eauto;
+              [exact msiSv_impl_ORqsInit
+              |exact msiSv_impl_RqRsSys
+              |red; auto
+              |exact msiSvMsgOutPred_good].
+          * repeat (constructor; simpl).
+        + destruct H6; split.
+          * red in H6; red; simpl in *; mred; simpl.
+            destruct (oss@[child2Idx]) as [cost2|]; simpl in *; [|auto].
+            destruct (orqs@[child2Idx]) as [corq2|]; simpl in *; [|auto].
+            destruct H6 as [[cv ?] ?].
+            red in H6; dest.
+            split.
+            { exists val0.
+              red; repeat ssplit.
+              { solve_rule_conds_ex; solve_msi. }
+              { solve_rule_conds_ex. }
+              { solve_rule_conds_ex; solve_msi. }
+              { solve_rule_conds_ex; solve_msi. }
             }
-            { repeat (constructor; simpl). }
-          * red; simpl; intros.
-            icase oidx.
-            { repeat (simpl; red; mred). }
-            { mred; apply H7; auto. }
-        + red in H6; red; simpl in *; mred; simpl.
-          destruct (oss@[child2Idx]) as [cost2|]; simpl in *; [|auto].
-          destruct (orqs@[child2Idx]) as [corq2|]; simpl in *; [|auto].
-          destruct H6 as [[cv ?] ?].
-          red in H6; dest.
-          split.
-          * exists val0.
-            red; repeat ssplit.
             { solve_rule_conds_ex; solve_msi. }
-            { solve_rule_conds_ex. }
-            { solve_rule_conds_ex; solve_msi. }
-            { solve_rule_conds_ex; solve_msi. }
-          * solve_rule_conds_ex; solve_msi.
-
+          * red in H22; red; simpl in *; mred.
+            
       - (** [childDownRqS] *)
         disc_rule_conds_ex.
 
         (* construction *)
         split.
-        + split.
-          * apply Forall_app.
-            { apply forall_removeOnce.
-              eapply atomic_rqDown_preserves_msg_out_preds; eauto;
-                [exact msiSv_impl_ORqsInit
-                |exact msiSv_impl_RqRsSys
-                |red; auto
-                |exact msiSvMsgOutPred_good].
+        + apply Forall_app.
+          * apply forall_removeOnce.
+            eapply atomic_rqDown_preserves_msg_out_preds; eauto;
+              [exact msiSv_impl_ORqsInit
+              |exact msiSv_impl_RqRsSys
+              |red; auto
+              |exact msiSvMsgOutPred_good].
+          * repeat (constructor; simpl).
+            red; simpl.
+            mred; simpl; auto.
+        + destruct H6; split.
+          * red in H6; red; simpl in *; mred; simpl.
+            destruct (oss@[parentIdx]) as [post|] eqn:Hpost; simpl in *; [|auto].
+            destruct (oss@[child2Idx]) as [cost2|] eqn:Hcost2; simpl in *; [|auto].
+            destruct (orqs@[child2Idx]) as [corq2|] eqn:Hcorq2; simpl in *; [|auto].
+            destruct H6 as [[cv ?] ?].
+            red in H6; dest.
+            split.
+            { exists cv.
+              red; repeat ssplit.
+              { solve_rule_conds_ex. }
+              { solve_rule_conds_ex. }
+              { solve_rule_conds_ex. }
+              { solve_rule_conds_ex; solve_msi. }
             }
-            { repeat (constructor; simpl).
-              red; simpl.
-              mred; simpl; auto.
-            }
-          * red; simpl; intros.
-            icase oidx.
-            { mred. }
-            { mred; apply H7; auto. }
-        + red in H6; red; simpl in *; mred; simpl.
-          destruct (oss@[parentIdx]) as [post|] eqn:Hpost; simpl in *; [|auto].
-          destruct (oss@[child2Idx]) as [cost2|] eqn:Hcost2; simpl in *; [|auto].
-          destruct (orqs@[child2Idx]) as [corq2|] eqn:Hcorq2; simpl in *; [|auto].
-          destruct H6 as [[cv ?] ?].
-          red in H6; dest.
-          split.
-          * exists cv.
-            red; repeat ssplit.
-            { solve_rule_conds_ex. }
-            { solve_rule_conds_ex. }
-            { solve_rule_conds_ex. }
             { solve_rule_conds_ex; solve_msi. }
-          * solve_rule_conds_ex; solve_msi.
+          * red in H7; red; simpl in *; mred.
 
       - atomic_cont_exfalso_bound MsiSvMsgOutPred.
       - atomic_cont_exfalso_bound MsiSvMsgOutPred.
@@ -679,89 +764,77 @@ Section Inv.
         good_footprint_get child1Idx.
         disc_rule_conds_ex.
 
-        (* discharge lock predicates *)
-        obj_visited_rsDown child1Idx.
-        disc_lock_preds child1Idx.
-        disc_rule_conds_ex.
-
         (* discharge message predicates *)
         disc_msg_preds H4.
         disc_rule_conds_ex.
 
         (* generate hints for leaves (L1 caches) *)
-        pose proof (parentIdxOf_child_indsOf _ _ H8).
+        pose proof (parentIdxOf_child_indsOf _ _ H7).
         dest_in; try discriminate; simpl in *.
-        cbn in H27; inv H27.
+        cbn in H26; inv H26.
 
         (* construction *)
         split.
-        + split.
-          * apply Forall_app.
-            { apply forall_removeOnce.
-              eapply atomic_rsDown_preserves_msg_out_preds; eauto;
-                [exact msiSv_impl_ORqsInit
-                |exact msiSv_impl_RqRsSys
-                |red; auto
-                |exact msiSvMsgOutPred_good].
+        + apply Forall_app.
+          * apply forall_removeOnce.
+            eapply atomic_rsDown_preserves_msg_out_preds; eauto;
+              [exact msiSv_impl_ORqsInit
+              |exact msiSv_impl_RqRsSys
+              |red; auto
+              |exact msiSvMsgOutPred_good].
+          * repeat (constructor; simpl).
+        + destruct H6; split.
+          * red in H6; red; simpl in *; mred; simpl.
+            destruct (oss@[child2Idx]) as [cost2|]; simpl in *; [|auto].
+            destruct (orqs@[child2Idx]) as [corq2|]; simpl in *; [|auto].
+            destruct H6 as [[cv ?] ?].
+            red in H6; dest.
+            split.
+            { exists n.
+              red; repeat ssplit.
+              { solve_rule_conds_ex.
+                destruct H6 as [|[|]]; try (exfalso; dest; discriminate).
+                right; right; solve_rule_conds_ex.
+              }
+              { solve_rule_conds_ex. }
+              { solve_rule_conds_ex; solve_msi. }
+              { solve_rule_conds_ex; solve_msi. }
             }
-            { repeat (constructor; simpl). }
-          * red; simpl; intros.
-            icase oidx.
-            { repeat (simpl; red; mred). }
-            { mred; apply H7; auto. }
-        + red in H6; red; simpl in *; mred; simpl.
-          destruct (oss@[child2Idx]) as [cost2|]; simpl in *; [|auto].
-          destruct (orqs@[child2Idx]) as [corq2|]; simpl in *; [|auto].
-          destruct H6 as [[cv ?] ?].
-          red in H6; dest.
-          split.
-          * exists n.
-            red; repeat ssplit.
-            { solve_rule_conds_ex.
-              destruct H6 as [|[|]]; try (exfalso; dest; discriminate).
-              right; right; solve_rule_conds_ex.
-            }
-            { solve_rule_conds_ex. }
             { solve_rule_conds_ex; solve_msi. }
-            { solve_rule_conds_ex; solve_msi. }
-          * solve_rule_conds_ex; solve_msi.
+          * red in H22; red; simpl in *; mred.
 
       - (** [childDownRqM] *)
         disc_rule_conds_ex.
 
         (* construction *)
         split.
-        + split.
-          * apply Forall_app.
-            { apply forall_removeOnce.
-              eapply atomic_rqDown_preserves_msg_out_preds; eauto;
-                [exact msiSv_impl_ORqsInit
-                |exact msiSv_impl_RqRsSys
-                |red; auto
-                |exact msiSvMsgOutPred_good].
+        + apply Forall_app.
+          * apply forall_removeOnce.
+            eapply atomic_rqDown_preserves_msg_out_preds; eauto;
+              [exact msiSv_impl_ORqsInit
+              |exact msiSv_impl_RqRsSys
+              |red; auto
+              |exact msiSvMsgOutPred_good].
+          * repeat (constructor; simpl).
+            red; simpl.
+            mred; simpl; auto.
+        + destruct H6; split.
+          * red in H6; red; simpl in *; mred; simpl.
+            destruct (oss@[parentIdx]) as [post|] eqn:Hpost; simpl in *; [|auto].
+            destruct (oss@[child2Idx]) as [cost2|] eqn:Hcost2; simpl in *; [|auto].
+            destruct (orqs@[child2Idx]) as [corq2|] eqn:Hcorq2; simpl in *; [|auto].
+            destruct H6 as [[cv ?] ?].
+            red in H6; dest.
+            split.
+            { exists cv.
+              red; repeat ssplit.
+              { solve_rule_conds_ex. }
+              { solve_rule_conds_ex. }
+              { solve_rule_conds_ex. }
+              { solve_rule_conds_ex. }
             }
-            { repeat (constructor; simpl).
-              red; simpl.
-              mred; simpl; auto.
-            }
-          * red; simpl; intros.
-            icase oidx.
-            { mred. }
-            { mred; apply H7; auto. }
-        + red in H6; red; simpl in *; mred; simpl.
-          destruct (oss@[parentIdx]) as [post|] eqn:Hpost; simpl in *; [|auto].
-          destruct (oss@[child2Idx]) as [cost2|] eqn:Hcost2; simpl in *; [|auto].
-          destruct (orqs@[child2Idx]) as [corq2|] eqn:Hcorq2; simpl in *; [|auto].
-          destruct H6 as [[cv ?] ?].
-          red in H6; dest.
-          split.
-          * exists cv.
-            red; repeat ssplit.
-            { solve_rule_conds_ex. }
-            { solve_rule_conds_ex. }
-            { solve_rule_conds_ex. }
-            { solve_rule_conds_ex. }
-          * solve_rule_conds_ex; solve_msi.
+            { solve_rule_conds_ex; solve_msi. }
+          * red in H7; red; simpl in *; mred.
 
       - atomic_cont_exfalso_bound MsiSvMsgOutPred.
       - (** [childEvictRsI] *)
@@ -769,51 +842,42 @@ Section Inv.
         good_footprint_get child1Idx.
         disc_rule_conds_ex.
 
-        (* discharge lock predicates *)
-        obj_visited_rsDown child1Idx.
-        disc_lock_preds child1Idx.
-        disc_rule_conds_ex.
-
         (* discharge message predicates *)
         disc_msg_preds H4.
         disc_rule_conds_ex.
 
         (* generate hints for leaves (L1 caches) *)
-        pose proof (parentIdxOf_child_indsOf _ _ H8).
+        pose proof (parentIdxOf_child_indsOf _ _ H7).
         dest_in; try discriminate; simpl in *.
-        cbn in H22; inv H22.
+        cbn in H21; inv H21.
 
         (* construction *)
         split.
-        + split.
-          * apply Forall_app.
-            { apply forall_removeOnce.
-              eapply atomic_rsDown_preserves_msg_out_preds; eauto;
-                [exact msiSv_impl_ORqsInit
-                |exact msiSv_impl_RqRsSys
-                |red; auto
-                |exact msiSvMsgOutPred_good].
+        + apply Forall_app.
+          * apply forall_removeOnce.
+            eapply atomic_rsDown_preserves_msg_out_preds; eauto;
+              [exact msiSv_impl_ORqsInit
+              |exact msiSv_impl_RqRsSys
+              |red; auto
+              |exact msiSvMsgOutPred_good].
+          * repeat (constructor; simpl).
+        + destruct H6; split.
+          * red in H6; red; simpl in *; mred; simpl.
+            rename porq into orq.
+            destruct (oss@[child2Idx]) as [cost2|]; simpl in *; [|auto].
+            destruct (orqs@[child2Idx]) as [corq2|]; simpl in *; [|auto].
+            destruct H6 as [[cv ?] ?].
+            red in H6; dest.
+            split.
+            { exists cv.
+              red; repeat ssplit.
+              { solve_rule_conds_ex. }
+              { solve_rule_conds_ex; solve_msi. }
+              { solve_rule_conds_ex. }
+              { solve_rule_conds_ex. }
             }
-            { repeat (constructor; simpl). }
-          * red; simpl; intros.
-            icase oidx.
-            { repeat (simpl; red; mred). }
-            { mred; apply H7; auto. }
-        + red in H6; red; simpl in *; mred; simpl.
-          rename porq into orq.
-          destruct (oss@[child2Idx]) as [cost2|]; simpl in *; [|auto].
-          destruct (orqs@[child2Idx]) as [corq2|]; simpl in *; [|auto].
-          destruct H6 as [[cv ?] ?].
-          red in H6; dest.
-          split.
-          * exists cv.
-            clear H22.
-            red; repeat ssplit.
-            { solve_rule_conds_ex. }
             { solve_rule_conds_ex; solve_msi. }
-            { solve_rule_conds_ex. }
-            { solve_rule_conds_ex. }
-          * solve_rule_conds_ex; solve_msi.
+          * red in H20; red; simpl in *; mred.
 
       (** child2 *)
       - atomic_cont_exfalso_bound MsiSvMsgOutPred.
@@ -824,86 +888,74 @@ Section Inv.
         good_footprint_get child2Idx.
         disc_rule_conds_ex.
 
-        (* discharge lock predicates *)
-        obj_visited_rsDown child2Idx.
-        disc_lock_preds child2Idx.
-        disc_rule_conds_ex.
-
         (* discharge message predicates *)
         disc_msg_preds H4.
         disc_rule_conds_ex.
 
         (* generate hints for leaves (L1 caches) *)
-        pose proof (parentIdxOf_child_indsOf _ _ H8).
+        pose proof (parentIdxOf_child_indsOf _ _ H7).
         dest_in; try discriminate; simpl in *.
-        cbn in H27; inv H27.
+        cbn in H26; inv H26.
 
         (* construction *)
         split.
-        + split.
-          * apply Forall_app.
-            { apply forall_removeOnce.
-              eapply atomic_rsDown_preserves_msg_out_preds; eauto;
-                [exact msiSv_impl_ORqsInit
-                |exact msiSv_impl_RqRsSys
-                |red; auto
-                |exact msiSvMsgOutPred_good].
+        + apply Forall_app.
+          * apply forall_removeOnce.
+            eapply atomic_rsDown_preserves_msg_out_preds; eauto;
+              [exact msiSv_impl_ORqsInit
+              |exact msiSv_impl_RqRsSys
+              |red; auto
+              |exact msiSvMsgOutPred_good].
+          * repeat (constructor; simpl).
+        + destruct H6; split.
+          * red in H6; red; simpl in *; mred; simpl.
+            destruct (oss@[child1Idx]) as [cost1|]; simpl in *; [|auto].
+            destruct (orqs@[child1Idx]) as [corq1|]; simpl in *; [|auto].
+            destruct H6 as [[cv ?] ?].
+            red in H6; dest.
+            split.
+            { exists val0.
+              red; repeat ssplit.
+              { solve_rule_conds_ex; solve_msi. }
+              { solve_rule_conds_ex; solve_msi. }
+              { solve_rule_conds_ex. }
+              { solve_rule_conds_ex; solve_msi. }
             }
-            { repeat (constructor; simpl). }
-          * red; simpl; intros.
-            icase oidx.
-            { repeat (simpl; red; mred). }
-            { mred; apply H7; auto. }
-        + red in H6; red; simpl in *; mred; simpl.
-          destruct (oss@[child1Idx]) as [cost1|]; simpl in *; [|auto].
-          destruct (orqs@[child1Idx]) as [corq1|]; simpl in *; [|auto].
-          destruct H6 as [[cv ?] ?].
-          red in H6; dest.
-          split.
-          * exists val0.
-            red; repeat ssplit.
             { solve_rule_conds_ex; solve_msi. }
-            { solve_rule_conds_ex; solve_msi. }
-            { solve_rule_conds_ex. }
-            { solve_rule_conds_ex; solve_msi. }
-          * solve_rule_conds_ex; solve_msi.
+          * red in H22; red; simpl in *; mred.
 
       - (** [childDownRqS] *)
         disc_rule_conds_ex.
 
         (* construction *)
         split.
-        + split.
-          * apply Forall_app.
-            { apply forall_removeOnce.
-              eapply atomic_rqDown_preserves_msg_out_preds; eauto;
-                [exact msiSv_impl_ORqsInit
-                |exact msiSv_impl_RqRsSys
-                |red; auto
-                |exact msiSvMsgOutPred_good].
+        + apply Forall_app.
+          * apply forall_removeOnce.
+            eapply atomic_rqDown_preserves_msg_out_preds; eauto;
+              [exact msiSv_impl_ORqsInit
+              |exact msiSv_impl_RqRsSys
+              |red; auto
+              |exact msiSvMsgOutPred_good].
+          * repeat (constructor; simpl).
+            red; simpl.
+            mred; simpl; auto.
+        + destruct H6; split.
+          * red in H6; red; simpl in *; mred; simpl.
+            destruct (oss@[parentIdx]) as [post|] eqn:Hpost; simpl in *; [|auto].
+            destruct (oss@[child1Idx]) as [cost1|] eqn:Hcost1; simpl in *; [|auto].
+            destruct (orqs@[child1Idx]) as [corq1|] eqn:Hcorq1; simpl in *; [|auto].
+            destruct H6 as [[cv ?] [? ?]].
+            red in H6; dest.
+            split.
+            { exists cv.
+              red; repeat ssplit.
+              { solve_rule_conds_ex. }
+              { solve_rule_conds_ex. }
+              { solve_rule_conds_ex. }
+              { solve_rule_conds_ex; solve_msi. }
             }
-            { repeat (constructor; simpl).
-              red; simpl.
-              mred; simpl; auto.
-            }
-          * red; simpl; intros.
-            icase oidx.
-            { mred. }
-            { mred; apply H7; auto. }
-        + red in H6; red; simpl in *; mred; simpl.
-          destruct (oss@[parentIdx]) as [post|] eqn:Hpost; simpl in *; [|auto].
-          destruct (oss@[child1Idx]) as [cost1|] eqn:Hcost1; simpl in *; [|auto].
-          destruct (orqs@[child1Idx]) as [corq1|] eqn:Hcorq1; simpl in *; [|auto].
-          destruct H6 as [[cv ?] ?].
-          red in H6; dest.
-          split.
-          * exists cv.
-            red; repeat ssplit.
-            { solve_rule_conds_ex. }
-            { solve_rule_conds_ex. }
-            { solve_rule_conds_ex. }
             { solve_rule_conds_ex; solve_msi. }
-          * solve_rule_conds_ex; solve_msi.
+          * red in H7; red; simpl in *; mred.
         
       - atomic_cont_exfalso_bound MsiSvMsgOutPred.
       - atomic_cont_exfalso_bound MsiSvMsgOutPred.
@@ -912,89 +964,77 @@ Section Inv.
         good_footprint_get child2Idx.
         disc_rule_conds_ex.
 
-        (* discharge lock predicates *)
-        obj_visited_rsDown child2Idx.
-        disc_lock_preds child2Idx.
-        disc_rule_conds_ex.
-
         (* discharge message predicates *)
         disc_msg_preds H4.
         disc_rule_conds_ex.
 
         (* generate hints for leaves (L1 caches) *)
-        pose proof (parentIdxOf_child_indsOf _ _ H8).
+        pose proof (parentIdxOf_child_indsOf _ _ H7).
         dest_in; try discriminate; simpl in *.
-        cbn in H27; inv H27.
+        cbn in H26; inv H26.
 
         (* construction *)
         split.
-        + split.
-          * apply Forall_app.
-            { apply forall_removeOnce.
-              eapply atomic_rsDown_preserves_msg_out_preds; eauto;
-                [exact msiSv_impl_ORqsInit
-                |exact msiSv_impl_RqRsSys
-                |red; auto
-                |exact msiSvMsgOutPred_good].
-            }
-            { repeat (constructor; simpl). }
-          * red; simpl; intros.
-            icase oidx.
-            { repeat (simpl; red; mred). }
-            { mred; apply H7; auto. }
-        + red in H6; red; simpl in *; mred; simpl.
-          destruct (oss@[child1Idx]) as [cost1|]; simpl in *; [|auto].
-          destruct (orqs@[child1Idx]) as [corq1|]; simpl in *; [|auto].
-          destruct H6 as [[cv ?] ?].
-          red in H6; dest.
-          split.
-          * exists n.
-            red; repeat ssplit.
-            { solve_rule_conds_ex.
-              destruct H6 as [|[|]]; try (exfalso; dest; discriminate).
-              right; right; solve_rule_conds_ex.
+        + apply Forall_app.
+          * apply forall_removeOnce.
+            eapply atomic_rsDown_preserves_msg_out_preds; eauto;
+              [exact msiSv_impl_ORqsInit
+              |exact msiSv_impl_RqRsSys
+              |red; auto
+              |exact msiSvMsgOutPred_good].
+          * repeat (constructor; simpl).
+        + destruct H6; split.
+          * red in H6; red; simpl in *; mred; simpl.
+            destruct (oss@[child1Idx]) as [cost1|]; simpl in *; [|auto].
+            destruct (orqs@[child1Idx]) as [corq1|]; simpl in *; [|auto].
+            destruct H6 as [[cv ?] ?].
+            red in H6; dest.
+            split.
+            { exists n.
+              red; repeat ssplit.
+              { solve_rule_conds_ex.
+                destruct H6 as [|[|]]; try (exfalso; dest; discriminate).
+                right; right; solve_rule_conds_ex.
+              }
+              { solve_rule_conds_ex; solve_msi. }
+              { solve_rule_conds_ex. }
+              { solve_rule_conds_ex; solve_msi. }
             }
             { solve_rule_conds_ex; solve_msi. }
-            { solve_rule_conds_ex. }
-            { solve_rule_conds_ex; solve_msi. }
-          * solve_rule_conds_ex; solve_msi.
+          * red in H22; red; simpl in *; mred.
           
       - (** [childDownRqM] *)
         disc_rule_conds_ex.
 
         (* construction *)
         split.
-        + split.
-          * apply Forall_app.
-            { apply forall_removeOnce.
-              eapply atomic_rqDown_preserves_msg_out_preds; eauto;
-                [exact msiSv_impl_ORqsInit
-                |exact msiSv_impl_RqRsSys
-                |red; auto
-                |exact msiSvMsgOutPred_good].
+        + apply Forall_app.
+          * apply forall_removeOnce.
+            eapply atomic_rqDown_preserves_msg_out_preds; eauto;
+              [exact msiSv_impl_ORqsInit
+              |exact msiSv_impl_RqRsSys
+              |red; auto
+              |exact msiSvMsgOutPred_good].
+          * repeat (constructor; simpl).
+            red; simpl.
+            mred; simpl; auto.
+        + destruct H6; split.
+          * red in H6; red; simpl in *; mred; simpl.
+            destruct (oss@[parentIdx]) as [post|] eqn:Hpost; simpl in *; [|auto].
+            destruct (oss@[child1Idx]) as [cost1|] eqn:Hcost1; simpl in *; [|auto].
+            destruct (orqs@[child1Idx]) as [corq1|] eqn:Hcorq1; simpl in *; [|auto].
+            destruct H6 as [[cv ?] [? ?]].
+            red in H6; dest.
+            split.
+            { exists cv.
+              red; repeat ssplit.
+              { solve_rule_conds_ex. }
+              { solve_rule_conds_ex. }
+              { solve_rule_conds_ex. }
+              { solve_rule_conds_ex. }
             }
-            { repeat (constructor; simpl).
-              red; simpl.
-              mred; simpl; auto.
-            }
-          * red; simpl; intros.
-            icase oidx.
-            { mred. }
-            { mred; apply H7; auto. }
-        + red in H6; red; simpl in *; mred; simpl.
-          destruct (oss@[parentIdx]) as [post|] eqn:Hpost; simpl in *; [|auto].
-          destruct (oss@[child1Idx]) as [cost1|] eqn:Hcost1; simpl in *; [|auto].
-          destruct (orqs@[child1Idx]) as [corq1|] eqn:Hcorq1; simpl in *; [|auto].
-          destruct H6 as [[cv ?] ?].
-          red in H6; dest.
-          split.
-          * exists cv.
-            red; repeat ssplit.
-            { solve_rule_conds_ex. }
-            { solve_rule_conds_ex. }
-            { solve_rule_conds_ex. }
-            { solve_rule_conds_ex. }
-          * solve_rule_conds_ex; solve_msi.
+            { solve_rule_conds_ex; solve_msi. }
+          * red in H7; red; simpl in *; mred.
 
       - atomic_cont_exfalso_bound MsiSvMsgOutPred.
       - (** [childEvictRsI] *)
@@ -1002,49 +1042,42 @@ Section Inv.
         good_footprint_get child2Idx.
         disc_rule_conds_ex.
 
-        (* discharge lock predicates *)
-        obj_visited_rsDown child2Idx.
-        disc_lock_preds child2Idx.
-        disc_rule_conds_ex.
-
         (* discharge message predicates *)
         disc_msg_preds H4.
         disc_rule_conds_ex.
 
         (* generate hints for leaves (L1 caches) *)
-        pose proof (parentIdxOf_child_indsOf _ _ H8).
+        pose proof (parentIdxOf_child_indsOf _ _ H7).
         dest_in; try discriminate; simpl in *.
-        cbn in H22; inv H22.
+        cbn in H21; inv H21.
 
         (* construction *)
         split.
-        + split.
-          * apply Forall_app.
-            { apply forall_removeOnce.
-              eapply atomic_rsDown_preserves_msg_out_preds; eauto;
-                [exact msiSv_impl_ORqsInit
-                |exact msiSv_impl_RqRsSys
-                |red; auto
-                |exact msiSvMsgOutPred_good].
+        + apply Forall_app.
+          * apply forall_removeOnce.
+            eapply atomic_rsDown_preserves_msg_out_preds; eauto;
+              [exact msiSv_impl_ORqsInit
+              |exact msiSv_impl_RqRsSys
+              |red; auto
+              |exact msiSvMsgOutPred_good].
+          * repeat (constructor; simpl).
+        + destruct H6; split.
+          * red in H6; red; simpl in *; mred; simpl.
+            rename porq into orq.
+            destruct (oss@[child1Idx]) as [cost1|]; simpl in *; [|auto].
+            destruct (orqs@[child1Idx]) as [corq1|]; simpl in *; [|auto].
+            destruct H6 as [[cv ?] ?].
+            red in H6; dest.
+            split.
+            { exists cv.
+              red; repeat ssplit.
+              { solve_rule_conds_ex. }
+              { solve_rule_conds_ex. }
+              { solve_rule_conds_ex; solve_msi. }
+              { solve_rule_conds_ex. }
             }
-            { repeat (constructor; simpl). }
-          * red; simpl; intros.
-            icase oidx.
-            { repeat (simpl; red; mred). }
-            { mred; apply H7; auto. }
-        + red in H6; red; simpl in *; mred; simpl.
-          destruct (oss@[child1Idx]) as [cost1|]; simpl in *; [|auto].
-          destruct (orqs@[child1Idx]) as [corq1|]; simpl in *; [|auto].
-          destruct H6 as [[cv ?] ?].
-          red in H6; dest.
-          split.
-          * exists cv.
-            red; repeat ssplit.
-            { solve_rule_conds_ex. }
-            { solve_rule_conds_ex. }
             { solve_rule_conds_ex; solve_msi. }
-            { solve_rule_conds_ex. }
-          * solve_rule_conds_ex; solve_msi.
+          * red in H20; red; simpl in *; mred.
 
       (** parent(child1) *)
 
@@ -1052,286 +1085,261 @@ Section Inv.
         disc_rule_conds_ex.
 
         split.
-        + split.
-          * apply Forall_app.
-            { apply forall_removeOnce.
-              eapply atomic_rqUp_preserves_msg_out_preds with (oidx:= child1Idx);
-                [exact msiSv_impl_ORqsInit
-                |exact msiSv_impl_RqRsSys|..]; eauto.
-              { intro; dest_in; discriminate. }
-              { red; auto. }
-              { exact msiSvMsgOutPred_good. }
-            }
-            { repeat (constructor; simpl).
-              red; repeat (simpl; mred).
-            }
-          * red; simpl; intros.
-            icase oidx.
-            { repeat (simpl; red; mred). }
-            { mred; apply H7; auto. }
-        + red in H6; red; simpl in *; mred; simpl.
-          destruct (oss@[child1Idx]) as [cost1|] eqn:Hcost1; simpl in *; [|auto].
-          destruct (oss@[child2Idx]) as [cost2|] eqn:Hcost2; simpl in *; [|auto].
-          destruct (orqs@[child1Idx]) as [corq1|] eqn:Hcorq1; simpl in *; [|auto].
-          destruct (orqs@[child2Idx]) as [corq2|] eqn:Hcorq2; simpl in *; [|auto].
-          destruct H6 as [[cv ?] ?].
-          red in H6; dest.
-          split.
-          * exists cv.
-            clear H8.
-            red; repeat ssplit.
-            { solve_rule_conds_ex.
-              right; left.
-              destruct H6 as [|[|]].
-              { solve_rule_conds_ex; solve_msi. }
+        + apply Forall_app.
+          * apply forall_removeOnce.
+            eapply atomic_rqUp_preserves_msg_out_preds with (oidx:= child1Idx);
+              [exact msiSv_impl_ORqsInit
+              |exact msiSv_impl_RqRsSys|..]; eauto.
+            { intro; dest_in; discriminate. }
+            { red; auto. }
+            { exact msiSvMsgOutPred_good. }
+          * repeat (constructor; simpl).
+            red; repeat (simpl; mred).
+        + destruct H6; split.
+          * red in H6; red; simpl in *; mred; simpl.
+            destruct (oss@[child1Idx]) as [cost1|] eqn:Hcost1; simpl in *; [|auto].
+            destruct (oss@[child2Idx]) as [cost2|] eqn:Hcost2; simpl in *; [|auto].
+            destruct (orqs@[child1Idx]) as [corq1|] eqn:Hcorq1; simpl in *; [|auto].
+            destruct (orqs@[child2Idx]) as [corq2|] eqn:Hcorq2; simpl in *; [|auto].
+            destruct H6 as [[cv ?] ?].
+            red in H6; dest.
+            split.
+            { exists cv.
+              red; repeat ssplit.
+              { solve_rule_conds_ex.
+                right; left.
+                destruct H6 as [|[|]].
+                { solve_rule_conds_ex; solve_msi. }
+                { solve_rule_conds_ex. }
+                { solve_msi. }
+              }
               { solve_rule_conds_ex. }
-              { solve_msi. }
+              { solve_rule_conds_ex. }
+              { solve_rule_conds_ex. }
             }
-            { solve_rule_conds_ex. }
-            { solve_rule_conds_ex. }
-            { solve_rule_conds_ex. }
-          * disc_rule_conds_ex.
-            assert (In (child child1Idx ec1 ce1 c1pRq c1pRs pc1) (sys_objs impl))
-              by (simpl; tauto).
-            good_locking_get (child child1Idx ec1 ce1 c1pRq c1pRs pc1).
-            clear H24.
-            eapply upLockInvORq_rqUp_length_one_locked in H26; try reflexivity;
-              [|eapply findQ_length_ge_one; apply FirstMP_InMP; eassumption].
-            solve_rule_conds_ex.
+            { disc_rule_conds_ex.
+              assert (In (child child1Idx ec1 ce1 c1pRq c1pRs pc1) (sys_objs impl))
+                by (simpl; tauto).
+              good_locking_get (child child1Idx ec1 ce1 c1pRq c1pRs pc1).
+              clear H24.
+              eapply upLockInvORq_rqUp_length_one_locked in H26; try reflexivity;
+                [|eapply findQ_length_ge_one; apply FirstMP_InMP; eassumption].
+              solve_rule_conds_ex.
+            }
+          * red in H7; red; simpl in *; mred.
 
       - (** [parentGetDownRqS] *)
         disc_rule_conds_ex.
 
         split.
-        + split.
-          * apply Forall_app.
-            { apply forall_removeOnce.
-              eapply atomic_rqUp_preserves_msg_out_preds with (oidx:= child1Idx);
-                [exact msiSv_impl_ORqsInit
-                |exact msiSv_impl_RqRsSys|..]; eauto.
-              { intro; dest_in; discriminate. }
-              { red; auto. }
-              { exact msiSvMsgOutPred_good. }
-            }
-            { repeat (constructor; simpl). }
-          * red; simpl; intros.
-            icase oidx.
-            { repeat (simpl; red; mred).
-              simpl; left; auto.
-            }
-            { mred; apply H7; auto. }
-        + red in H6; red; simpl in *; mred.
+        + apply Forall_app.
+          * apply forall_removeOnce.
+            eapply atomic_rqUp_preserves_msg_out_preds with (oidx:= child1Idx);
+              [exact msiSv_impl_ORqsInit
+              |exact msiSv_impl_RqRsSys|..]; eauto.
+            { intro; dest_in; discriminate. }
+            { red; auto. }
+            { exact msiSvMsgOutPred_good. }
+          * repeat (constructor; simpl).
+        + destruct H6; split.
+          * red in H6; red; simpl in *; mred.
+          * solve_rule_conds_ex.
 
       - (** [parentSetRqImm] *)
         disc_rule_conds_ex.
 
         split.
-        + split.
-          * apply Forall_app.
-            { apply forall_removeOnce.
-              eapply atomic_rqUp_preserves_msg_out_preds with (oidx:= child1Idx);
-                [exact msiSv_impl_ORqsInit
-                |exact msiSv_impl_RqRsSys|..]; eauto.
-              { intro; dest_in; discriminate. }
-              { red; auto. }
-              { exact msiSvMsgOutPred_good. }
-            }
-            { repeat (constructor; simpl).
-              red; repeat (simpl; mred).
-            }
-          * red; simpl; intros.
-            icase oidx.
-            { repeat (simpl; red; mred). }
-            { mred; apply H7; auto. }
-        + red in H6; red; simpl in *; mred; simpl.
-          destruct (oss@[child1Idx]) as [cost1|] eqn:Hcost1; simpl in *; [|auto].
-          destruct (oss@[child2Idx]) as [cost2|] eqn:Hcost2; simpl in *; [|auto].
-          destruct (orqs@[child1Idx]) as [corq1|] eqn:Hcorq1; simpl in *; [|auto].
-          destruct (orqs@[child2Idx]) as [corq2|] eqn:Hcorq2; simpl in *; [|auto].
-          destruct H6 as [[cv ?] ?].
-          red in H6; dest.
-          unfold getDir in H14; simpl in H14.
+        + apply Forall_app.
+          * apply forall_removeOnce.
+            eapply atomic_rqUp_preserves_msg_out_preds with (oidx:= child1Idx);
+              [exact msiSv_impl_ORqsInit
+              |exact msiSv_impl_RqRsSys|..]; eauto.
+            { intro; dest_in; discriminate. }
+            { red; auto. }
+            { exact msiSvMsgOutPred_good. }
+          * repeat (constructor; simpl).
+            red; repeat (simpl; mred).
+        + destruct H6; split.
+          * red in H6; red; simpl in *; mred; simpl.
+            destruct (oss@[child1Idx]) as [cost1|] eqn:Hcost1; simpl in *; [|auto].
+            destruct (oss@[child2Idx]) as [cost2|] eqn:Hcost2; simpl in *; [|auto].
+            destruct (orqs@[child1Idx]) as [corq1|] eqn:Hcorq1; simpl in *; [|auto].
+            destruct (orqs@[child2Idx]) as [corq2|] eqn:Hcorq2; simpl in *; [|auto].
+            destruct H6 as [[cv ?] ?].
+            red in H6; dest.
+            unfold getDir in H13; simpl in H13.
 
-          split.
-          * exists cv.
-            red; repeat ssplit.
-            { solve_rule_conds_ex.
-              right; right; auto.
+            split.
+            { exists cv.
+              red; repeat ssplit.
+              { solve_rule_conds_ex.
+                right; right; auto.
+              }
+              { solve_rule_conds_ex. }
+              { solve_rule_conds_ex. }
+              { solve_rule_conds_ex. }
             }
-            { solve_rule_conds_ex. }
-            { solve_rule_conds_ex. }
-            { solve_rule_conds_ex. }
-          * disc_rule_conds_ex.
-            assert (In (child child1Idx ec1 ce1 c1pRq c1pRs pc1) (sys_objs impl))
-              by (simpl; tauto).
-            good_locking_get (child child1Idx ec1 ce1 c1pRq c1pRs pc1).
-            clear H24.
-            eapply upLockInvORq_rqUp_length_one_locked in H26; try reflexivity;
-              [|eapply findQ_length_ge_one; apply FirstMP_InMP; eassumption].
-            solve_rule_conds_ex.
+            { disc_rule_conds_ex.
+              assert (In (child child1Idx ec1 ce1 c1pRq c1pRs pc1) (sys_objs impl))
+                by (simpl; tauto).
+              good_locking_get (child child1Idx ec1 ce1 c1pRq c1pRs pc1).
+              clear H24.
+              eapply upLockInvORq_rqUp_length_one_locked in H26; try reflexivity;
+                [|eapply findQ_length_ge_one; apply FirstMP_InMP; eassumption].
+              solve_rule_conds_ex.
+            }
+          * red in H7; red; simpl in *; mred.
 
       - (** [parentSetDownRqM] *)
         disc_rule_conds_ex.
 
         split.
-        + split.
-          * apply Forall_app.
-            { apply forall_removeOnce.
-              eapply atomic_rqUp_preserves_msg_out_preds with (oidx:= child1Idx);
-                [exact msiSv_impl_ORqsInit
-                |exact msiSv_impl_RqRsSys|..]; eauto.
-              { intro; dest_in; discriminate. }
-              { red; auto. }
-              { exact msiSvMsgOutPred_good. }
-            }
-            { repeat (constructor; simpl). }
-          * red; simpl; intros.
-            icase oidx.
-            { repeat (simpl; red; mred).
-              simpl; left; auto.
-            }
-            { mred; apply H7; auto. }
-        + red in H6; red; simpl in *; mred.
+        + apply Forall_app.
+          * apply forall_removeOnce.
+            eapply atomic_rqUp_preserves_msg_out_preds with (oidx:= child1Idx);
+              [exact msiSv_impl_ORqsInit
+              |exact msiSv_impl_RqRsSys|..]; eauto.
+            { intro; dest_in; discriminate. }
+            { red; auto. }
+            { exact msiSvMsgOutPred_good. }
+          * repeat (constructor; simpl).
+        + destruct H6; split.
+          * red in H6; red; simpl in *; mred.
+          * solve_rule_conds_ex.
 
       - (** [parentGetDownRsS] *)
         disc_rule_conds_ex.
 
-        obj_visited_rsUp parentIdx child2Idx.
-        disc_lock_preds parentIdx.
-        disc_rule_conds_ex.
-        destruct H11; dest; [|discriminate].
-        clear H11.
-        disc_rule_conds_ex.
+        (* discharge the lock invariant *)
+        destruct H6.
+        red in H8; simpl in H8.
+        disc_rule_conds_const.
+        red in H8.
+        disc_rule_conds_const.
+        destruct H8; dest; [|discriminate].
+        rewrite H10 in *.
 
         (* discharge message predicates *)
         disc_msg_preds H4.
         disc_rule_conds_ex.
         
         split.
-        + split.
-          * apply Forall_app.
-            { apply forall_removeOnce.
-              eapply atomic_rsUps_preserves_msg_out_preds
-                with (rsUps:= [(c2pRs, rmsg)]); eauto.
-              { exact msiSv_impl_ORqsInit. }
-              { exact msiSv_impl_RqRsSys. }
-              { repeat constructor; intro; dest_in. }
-              { apply SubList_cons; [|apply SubList_nil].
-                assumption.
-              }
-              { instantiate (1:= fun _ => True).
-                instantiate (1:= [pc2]).
+        + apply Forall_app.
+          * apply forall_removeOnce.
+            eapply atomic_rsUps_preserves_msg_out_preds
+              with (rsUps:= [(c2pRs, rmsg)]); eauto.
+            { exact msiSv_impl_ORqsInit. }
+            { exact msiSv_impl_RqRsSys. }
+            { repeat constructor; intro; dest_in. }
+            { apply SubList_cons; [|apply SubList_nil].
+              assumption.
+            }
+            { instantiate (1:= fun _ => True).
+              instantiate (1:= [pc2]).
+              repeat split.
+              { discriminate. }
+              { repeat constructor.
+                simpl; exists child2Idx.
                 repeat split.
-                { discriminate. }
-                { repeat constructor.
-                  simpl; exists child2Idx.
-                  repeat split.
-                }
               }
-              { exact msiSvMsgOutPred_good. }
             }
-            { repeat (constructor; simpl).
-              red; simpl.
-              solve_rule_conds_ex.
-            }
-          * red; simpl; intros.
-            icase oidx.
-            { repeat (simpl; red; mred). }
-            { mred; apply H7; auto. }
-        + red in H6; red; simpl in *; mred; simpl.
-          destruct (oss@[child1Idx]) as [cost1|] eqn:Hcost1; simpl in *; [|auto].
-          destruct (orqs@[child1Idx]) as [corq1|] eqn:Hcorq1; simpl in *; [|auto].
-          destruct (orqs@[child2Idx]) as [corq2|] eqn:Hcorq2; simpl in *; [|auto].
-          destruct H6 as [[cv ?] ?].
-          red in H6; dest.
+            { exact msiSvMsgOutPred_good. }
+          * repeat (constructor; simpl).
+            red; simpl.
+            solve_rule_conds_ex.
+        + split.
+          * red in H6; red; simpl in *; mred; simpl.
+            destruct (oss@[child1Idx]) as [cost1|] eqn:Hcost1; simpl in *; [|auto].
+            destruct (orqs@[child1Idx]) as [corq1|] eqn:Hcorq1; simpl in *; [|auto].
+            destruct (orqs@[child2Idx]) as [corq2|] eqn:Hcorq2; simpl in *; [|auto].
+            destruct H6 as [[cv ?] ?].
+            red in H6; dest.
 
-          assert (In (child child1Idx ec1 ce1 c1pRq c1pRs pc1) (sys_objs impl))
-            by (simpl; tauto).
-          good_locking_get (child child1Idx ec1 ce1 c1pRq c1pRs pc1).
-          clear H24.
-          eapply upLockInvORq_parent_locked_locked in H26; try reflexivity;
-            [|red; repeat (simpl; mred); eauto]; dest.
+            assert (In (child child1Idx ec1 ce1 c1pRq c1pRs pc1) (sys_objs impl))
+              by (simpl; tauto).
+            good_locking_get (child child1Idx ec1 ce1 c1pRq c1pRs pc1).
+            clear H21.
+            eapply upLockInvORq_parent_locked_locked in H22; try reflexivity;
+              [|red; repeat (simpl; mred); eauto]; dest.
           
-          split.
-          * exists val0.
-            clear H11.
-            red; repeat ssplit.
-            { solve_rule_conds_ex.
-              right; left; auto.
+            split.
+            { exists val0.
+              red; repeat ssplit.
+              { solve_rule_conds_ex.
+                right; left; auto.
+              }
+              { solve_rule_conds_ex. }
+              { solve_rule_conds_ex. }
+              { solve_rule_conds_ex. }
             }
-            { solve_rule_conds_ex. }
-            { solve_rule_conds_ex. }
             { solve_rule_conds_ex. }
           * solve_rule_conds_ex.
 
       - (** [parentSetDownRsM] *)
         disc_rule_conds_ex.
 
-        obj_visited_rsUp parentIdx child2Idx.
-        disc_lock_preds parentIdx.
-        disc_rule_conds_ex.
-        destruct H11; dest; [|discriminate].
-        clear H11.
-        disc_rule_conds_ex.
+        (* discharge the lock invariant *)
+        destruct H6.
+        red in H8; simpl in H8.
+        disc_rule_conds_const.
+        red in H8.
+        disc_rule_conds_const.
+        destruct H8; dest; [|discriminate].
+        rewrite H10 in *.
 
         (* discharge message predicates *)
         disc_msg_preds H4.
         disc_rule_conds_ex.
         
         split.
-        + split.
-          * apply Forall_app.
-            { apply forall_removeOnce.
-              eapply atomic_rsUps_preserves_msg_out_preds
-                with (rsUps:= [(c2pRs, rmsg)]); eauto.
-              { exact msiSv_impl_ORqsInit. }
-              { exact msiSv_impl_RqRsSys. }
-              { repeat constructor; intro; dest_in. }
-              { apply SubList_cons; [|apply SubList_nil].
-                assumption.
-              }
-              { instantiate (1:= fun _ => True).
-                instantiate (1:= [pc2]).
+        + apply Forall_app.
+          * apply forall_removeOnce.
+            eapply atomic_rsUps_preserves_msg_out_preds
+              with (rsUps:= [(c2pRs, rmsg)]); eauto.
+            { exact msiSv_impl_ORqsInit. }
+            { exact msiSv_impl_RqRsSys. }
+            { repeat constructor; intro; dest_in. }
+            { apply SubList_cons; [|apply SubList_nil].
+              assumption.
+            }
+            { instantiate (1:= fun _ => True).
+              instantiate (1:= [pc2]).
+              repeat split.
+              { discriminate. }
+              { repeat constructor.
+                simpl; exists child2Idx.
                 repeat split.
-                { discriminate. }
-                { repeat constructor.
-                  simpl; exists child2Idx.
-                  repeat split.
-                }
               }
-              { exact msiSvMsgOutPred_good. }
             }
-            { repeat (constructor; simpl).
-              red; simpl.
-              solve_rule_conds_ex.
-            }
-          * red; simpl; intros.
-            icase oidx.
-            { repeat (simpl; red; mred). }
-            { mred; apply H7; auto. }
-        + red in H6; red; simpl in *; mred; simpl.
-          destruct (oss@[child1Idx]) as [cost1|] eqn:Hcost1; simpl in *; [|auto].
-          destruct (orqs@[child1Idx]) as [corq1|] eqn:Hcorq1; simpl in *; [|auto].
-          destruct (orqs@[child2Idx]) as [corq2|] eqn:Hcorq2; simpl in *; [|auto].
-          destruct H6 as [[cv ?] ?].
-          red in H6; dest.
+            { exact msiSvMsgOutPred_good. }
+          * repeat (constructor; simpl).
+            red; simpl.
+            solve_rule_conds_ex.
+        + split.
+          * red in H6; red; simpl in *; mred; simpl.
+            destruct (oss@[child1Idx]) as [cost1|] eqn:Hcost1; simpl in *; [|auto].
+            destruct (orqs@[child1Idx]) as [corq1|] eqn:Hcorq1; simpl in *; [|auto].
+            destruct (orqs@[child2Idx]) as [corq2|] eqn:Hcorq2; simpl in *; [|auto].
+            destruct H6 as [[cv ?] ?].
+            red in H6; dest.
 
-          assert (In (child child1Idx ec1 ce1 c1pRq c1pRs pc1) (sys_objs impl))
-            by (simpl; tauto).
-          good_locking_get (child child1Idx ec1 ce1 c1pRq c1pRs pc1).
-          clear H24.
-          eapply upLockInvORq_parent_locked_locked in H26; try reflexivity;
-            [|red; repeat (simpl; mred); eauto]; dest.
+            assert (In (child child1Idx ec1 ce1 c1pRq c1pRs pc1) (sys_objs impl))
+              by (simpl; tauto).
+            good_locking_get (child child1Idx ec1 ce1 c1pRq c1pRs pc1).
+            clear H21.
+            eapply upLockInvORq_parent_locked_locked in H22; try reflexivity;
+              [|red; repeat (simpl; mred); eauto]; dest.
 
-          split.
-          * exists val0.
-            clear H11.
-            red; repeat ssplit.
-            { solve_rule_conds_ex.
-              right; right; auto.
+            split.
+            { exists val0.
+              red; repeat ssplit.
+              { solve_rule_conds_ex.
+                right; right; auto.
+              }
+              { solve_rule_conds_ex. }
+              { solve_rule_conds_ex. }
+              { solve_rule_conds_ex. }
             }
-            { solve_rule_conds_ex. }
-            { solve_rule_conds_ex. }
             { solve_rule_conds_ex. }
           * solve_rule_conds_ex.
 
@@ -1339,177 +1347,162 @@ Section Inv.
         disc_rule_conds_ex.
 
         split.
-        + split.
-          * apply Forall_app.
-            { apply forall_removeOnce.
-              eapply atomic_rqUp_preserves_msg_out_preds with (oidx:= child1Idx);
-                [exact msiSv_impl_ORqsInit
-                |exact msiSv_impl_RqRsSys|..]; eauto.
-              { intro; dest_in; discriminate. }
-              { red; auto. }
-              { exact msiSvMsgOutPred_good. }
-            }
-            { repeat (constructor; simpl).
-              red; repeat (simpl; mred).
-            }
-          * red; simpl; intros.
-            icase oidx.
-            { repeat (simpl; red; mred). }
-            { mred; apply H7; auto. }
-        + red in H6; red; simpl in *; mred.
+        + apply Forall_app.
+          * apply forall_removeOnce.
+            eapply atomic_rqUp_preserves_msg_out_preds with (oidx:= child1Idx);
+              [exact msiSv_impl_ORqsInit
+              |exact msiSv_impl_RqRsSys|..]; eauto.
+            { intro; dest_in; discriminate. }
+            { red; auto. }
+            { exact msiSvMsgOutPred_good. }
+          * repeat (constructor; simpl).
+            red; repeat (simpl; mred).
+        + destruct H6; split.
+          * red in H6; red; simpl in *; mred.
+          * red in H7; red; simpl in *; mred.
         
       - (** [parentEvictRqImmS] *)
         disc_rule_conds_ex.
 
         split.
-        + split.
-          * apply Forall_app.
-            { apply forall_removeOnce.
-              eapply atomic_rqUp_preserves_msg_out_preds with (oidx:= child1Idx);
-                [exact msiSv_impl_ORqsInit
-                |exact msiSv_impl_RqRsSys|..]; eauto.
-              { intro; dest_in; discriminate. }
-              { red; auto. }
-              { exact msiSvMsgOutPred_good. }
+        + apply Forall_app.
+          * apply forall_removeOnce.
+            eapply atomic_rqUp_preserves_msg_out_preds with (oidx:= child1Idx);
+              [exact msiSv_impl_ORqsInit
+              |exact msiSv_impl_RqRsSys|..]; eauto.
+            { intro; dest_in; discriminate. }
+            { red; auto. }
+            { exact msiSvMsgOutPred_good. }
+          * repeat (constructor; simpl).
+            red; repeat (simpl; mred).
+        + destruct H6; split.
+          * red in H6; red; simpl in *; mred; simpl.
+            destruct (oss@[child1Idx]) as [cost1|] eqn:Hcost1; simpl in *; [|auto].
+            destruct (oss@[child2Idx]) as [cost2|] eqn:Hcost2; simpl in *; [|auto].
+            destruct (orqs@[child1Idx]) as [corq1|] eqn:Hcorq1; simpl in *; [|auto].
+            destruct (orqs@[child2Idx]) as [corq2|] eqn:Hcorq2; simpl in *; [|auto].
+            destruct H6 as [[cv ?] ?].
+            red in H6; dest.
+            unfold getDir in *; simpl in *.
+            disc_rule_conds_ex.
+            destruct H6 as [|[|]];
+              [exfalso; solve_rule_conds_ex
+              | |exfalso; destruct H6 as [? [|]]; solve_rule_conds_ex].
+            split.
+            { exists cv.
+              repeat ssplit.
+              { solve_rule_conds_ex.
+                right; left; solve_msi.
+              }
+              { solve_rule_conds_ex. }
+              { solve_rule_conds_ex. }
+              { solve_rule_conds_ex. }
             }
-            { repeat (constructor; simpl).
-              red; repeat (simpl; mred).
+            { disc_rule_conds_ex.
+              assert (In (child child1Idx ec1 ce1 c1pRq c1pRs pc1) (sys_objs impl))
+                by (simpl; tauto).
+              good_locking_get (child child1Idx ec1 ce1 c1pRq c1pRs pc1).
+              clear H6.
+              eapply upLockInvORq_rqUp_length_one_locked in H28; try reflexivity;
+                [|eapply findQ_length_ge_one; apply FirstMP_InMP; eassumption].
+              solve_rule_conds_ex.
             }
-          * red; simpl; intros.
-            icase oidx.
-            { repeat (simpl; red; mred). }
-            { mred; apply H7; auto. }
-        + red in H6; red; simpl in *; mred; simpl.
-          destruct (oss@[child1Idx]) as [cost1|] eqn:Hcost1; simpl in *; [|auto].
-          destruct (oss@[child2Idx]) as [cost2|] eqn:Hcost2; simpl in *; [|auto].
-          destruct (orqs@[child1Idx]) as [corq1|] eqn:Hcorq1; simpl in *; [|auto].
-          destruct (orqs@[child2Idx]) as [corq2|] eqn:Hcorq2; simpl in *; [|auto].
-          destruct H6 as [[cv ?] ?].
-          red in H6; dest.
-          unfold getDir in *; simpl in *.
-          disc_rule_conds_ex.
-          destruct H6 as [|[|]];
-            [exfalso; solve_rule_conds_ex
-            | |exfalso; destruct H6 as [? [|]]; solve_rule_conds_ex].
-          split.
-          * exists cv.
-            repeat ssplit.
-            { solve_rule_conds_ex.
-              right; left; solve_msi.
-            }
-            { solve_rule_conds_ex. }
-            { solve_rule_conds_ex. }
-            { solve_rule_conds_ex. }
-          * disc_rule_conds_ex.
-            assert (In (child child1Idx ec1 ce1 c1pRq c1pRs pc1) (sys_objs impl))
-              by (simpl; tauto).
-            good_locking_get (child child1Idx ec1 ce1 c1pRq c1pRs pc1).
-            clear H6.
-            eapply upLockInvORq_rqUp_length_one_locked in H28; try reflexivity;
-              [|eapply findQ_length_ge_one; apply FirstMP_InMP; eassumption].
-            solve_rule_conds_ex.
+          * red in H7; red; simpl in *; mred.
 
       - (** [parentEvictRqImmLastS] *)
         disc_rule_conds_ex.
 
         split.
-        + split.
-          * apply Forall_app.
-            { apply forall_removeOnce.
-              eapply atomic_rqUp_preserves_msg_out_preds with (oidx:= child1Idx);
-                [exact msiSv_impl_ORqsInit
-                |exact msiSv_impl_RqRsSys|..]; eauto.
-              { intro; dest_in; discriminate. }
-              { red; auto. }
-              { exact msiSvMsgOutPred_good. }
+        + apply Forall_app.
+          * apply forall_removeOnce.
+            eapply atomic_rqUp_preserves_msg_out_preds with (oidx:= child1Idx);
+              [exact msiSv_impl_ORqsInit
+              |exact msiSv_impl_RqRsSys|..]; eauto.
+            { intro; dest_in; discriminate. }
+            { red; auto. }
+            { exact msiSvMsgOutPred_good. }
+          * repeat (constructor; simpl).
+            red; repeat (simpl; mred).
+        + destruct H6; split.
+          * red in H6; red; simpl in *; mred; simpl.
+            destruct (oss@[child1Idx]) as [cost1|] eqn:Hcost1; simpl in *; [|auto].
+            destruct (oss@[child2Idx]) as [cost2|] eqn:Hcost2; simpl in *; [|auto].
+            destruct (orqs@[child1Idx]) as [corq1|] eqn:Hcorq1; simpl in *; [|auto].
+            destruct (orqs@[child2Idx]) as [corq2|] eqn:Hcorq2; simpl in *; [|auto].
+            destruct H6 as [[cv ?] ?].
+            red in H6; dest.
+            unfold getDir in *; simpl in *.
+            disc_rule_conds_ex.
+            destruct H6 as [|[|]];
+              [exfalso; solve_rule_conds_ex
+              | |exfalso; destruct H6 as [? [|]]; solve_rule_conds_ex].
+            split.
+            { exists cv.
+              repeat ssplit.
+              { solve_rule_conds_ex.
+                left; auto.
+              }
+              { solve_rule_conds_ex. }
+              { solve_rule_conds_ex. }
+              { solve_rule_conds_ex. }
             }
-            { repeat (constructor; simpl).
-              red; repeat (simpl; mred).
+            { disc_rule_conds_ex.
+              assert (In (child child1Idx ec1 ce1 c1pRq c1pRs pc1) (sys_objs impl))
+                by (simpl; tauto).
+              good_locking_get (child child1Idx ec1 ce1 c1pRq c1pRs pc1).
+              clear H6.
+              eapply upLockInvORq_rqUp_length_one_locked in H28; try reflexivity;
+                [|eapply findQ_length_ge_one; apply FirstMP_InMP; eassumption].
+              solve_rule_conds_ex.
             }
-          * red; simpl; intros.
-            icase oidx.
-            { repeat (simpl; red; mred). }
-            { mred; apply H7; auto. }
-        + red in H6; red; simpl in *; mred; simpl.
-          destruct (oss@[child1Idx]) as [cost1|] eqn:Hcost1; simpl in *; [|auto].
-          destruct (oss@[child2Idx]) as [cost2|] eqn:Hcost2; simpl in *; [|auto].
-          destruct (orqs@[child1Idx]) as [corq1|] eqn:Hcorq1; simpl in *; [|auto].
-          destruct (orqs@[child2Idx]) as [corq2|] eqn:Hcorq2; simpl in *; [|auto].
-          destruct H6 as [[cv ?] ?].
-          red in H6; dest.
-          unfold getDir in *; simpl in *.
-          disc_rule_conds_ex.
-          destruct H6 as [|[|]];
-            [exfalso; solve_rule_conds_ex
-            | |exfalso; destruct H6 as [? [|]]; solve_rule_conds_ex].
-          split.
-          * exists cv.
-            repeat ssplit.
-            { solve_rule_conds_ex.
-              left; auto.
-            }
-            { solve_rule_conds_ex. }
-            { solve_rule_conds_ex. }
-            { solve_rule_conds_ex. }
-          * disc_rule_conds_ex.
-            assert (In (child child1Idx ec1 ce1 c1pRq c1pRs pc1) (sys_objs impl))
-              by (simpl; tauto).
-            good_locking_get (child child1Idx ec1 ce1 c1pRq c1pRs pc1).
-            clear H6.
-            eapply upLockInvORq_rqUp_length_one_locked in H28; try reflexivity;
-              [|eapply findQ_length_ge_one; apply FirstMP_InMP; eassumption].
-            solve_rule_conds_ex.
+          * red in H7; red; simpl in *; mred.
 
       - (** [parentEvictRqImmM] *)
         disc_rule_conds_ex.
 
         split.
-        + split.
-          * apply Forall_app.
-            { apply forall_removeOnce.
-              eapply atomic_rqUp_preserves_msg_out_preds with (oidx:= child1Idx);
-                [exact msiSv_impl_ORqsInit
-                |exact msiSv_impl_RqRsSys|..]; eauto.
-              { intro; dest_in; discriminate. }
-              { red; auto. }
-              { exact msiSvMsgOutPred_good. }
-            }
-            { repeat (constructor; simpl).
-              red; repeat (simpl; mred).
-            }
-          * red; simpl; intros.
-            icase oidx.
-            { repeat (simpl; red; mred). }
-            { mred; apply H7; auto. }
-        + red in H6; red; simpl in *; mred; simpl.
-          destruct (oss@[child1Idx]) as [cost1|] eqn:Hcost1; simpl in *; [|auto].
-          destruct (oss@[child2Idx]) as [cost2|] eqn:Hcost2; simpl in *; [|auto].
-          destruct (orqs@[child1Idx]) as [corq1|] eqn:Hcorq1; simpl in *; [|auto].
-          destruct (orqs@[child2Idx]) as [corq2|] eqn:Hcorq2; simpl in *; [|auto].
-          destruct H6 as [[cv ?] ?].
-          red in H6; dest.
-          unfold getDir in *; simpl in *.
-          disc_rule_conds_ex.
-          destruct H6 as [|[|]]; try (exfalso; solve_rule_conds_ex; fail).
+        + apply Forall_app.
+          * apply forall_removeOnce.
+            eapply atomic_rqUp_preserves_msg_out_preds with (oidx:= child1Idx);
+              [exact msiSv_impl_ORqsInit
+              |exact msiSv_impl_RqRsSys|..]; eauto.
+            { intro; dest_in; discriminate. }
+            { red; auto. }
+            { exact msiSvMsgOutPred_good. }
+          * repeat (constructor; simpl).
+            red; repeat (simpl; mred).
+        + destruct H6; split.
+          * red in H6; red; simpl in *; mred; simpl.
+            destruct (oss@[child1Idx]) as [cost1|] eqn:Hcost1; simpl in *; [|auto].
+            destruct (oss@[child2Idx]) as [cost2|] eqn:Hcost2; simpl in *; [|auto].
+            destruct (orqs@[child1Idx]) as [corq1|] eqn:Hcorq1; simpl in *; [|auto].
+            destruct (orqs@[child2Idx]) as [corq2|] eqn:Hcorq2; simpl in *; [|auto].
+            destruct H6 as [[cv ?] ?].
+            red in H6; dest.
+            unfold getDir in *; simpl in *.
+            disc_rule_conds_ex.
+            destruct H6 as [|[|]]; try (exfalso; solve_rule_conds_ex; fail).
 
-          assert (In (child child1Idx ec1 ce1 c1pRq c1pRs pc1) (sys_objs impl))
-            by (simpl; tauto).
-          good_locking_get (child child1Idx ec1 ce1 c1pRq c1pRs pc1).
-          clear H26.
-          eapply upLockInvORq_rqUp_length_one_locked in H27; try reflexivity;
-            [|eapply findQ_length_ge_one; apply FirstMP_InMP; eassumption].
-          disc_rule_conds_ex.
+            assert (In (child child1Idx ec1 ce1 c1pRq c1pRs pc1) (sys_objs impl))
+              by (simpl; tauto).
+            good_locking_get (child child1Idx ec1 ce1 c1pRq c1pRs pc1).
+            clear H26.
+            eapply upLockInvORq_rqUp_length_one_locked in H27; try reflexivity;
+              [|eapply findQ_length_ge_one; apply FirstMP_InMP; eassumption].
+            disc_rule_conds_ex.
           
-          split.
-          * exists n.
-            repeat ssplit.
-            { solve_rule_conds_ex.
-              left; solve_msi.
+            split.
+            { exists n.
+              repeat ssplit.
+              { solve_rule_conds_ex.
+                left; solve_msi.
+              }
+              { solve_rule_conds_ex. }
+              { solve_rule_conds_ex; solve_msi. }
+              { solve_rule_conds_ex. }
             }
             { solve_rule_conds_ex. }
-            { solve_rule_conds_ex; solve_msi. }
-            { solve_rule_conds_ex. }
-          * solve_rule_conds_ex.
+          * red in H7; red; simpl in *; mred.
 
       (** parent(child2) *)
 
@@ -1517,285 +1510,260 @@ Section Inv.
         disc_rule_conds_ex.
 
         split.
-        + split.
-          * apply Forall_app.
-            { apply forall_removeOnce.
-              eapply atomic_rqUp_preserves_msg_out_preds with (oidx:= child2Idx);
-                [exact msiSv_impl_ORqsInit
-                |exact msiSv_impl_RqRsSys|..]; eauto.
-              { intro; dest_in; discriminate. }
-              { red; auto. }
-              { exact msiSvMsgOutPred_good. }
-            }
-            { repeat (constructor; simpl).
-              red; repeat (simpl; mred).
-            }
-          * red; simpl; intros.
-            icase oidx.
-            { repeat (simpl; red; mred). }
-            { mred; apply H7; auto. }
-        + red in H6; red; simpl in *; mred; simpl.
-          destruct (oss@[child1Idx]) as [cost1|] eqn:Hcost1; simpl in *; [|auto].
-          destruct (oss@[child2Idx]) as [cost2|] eqn:Hcost2; simpl in *; [|auto].
-          destruct (orqs@[child1Idx]) as [corq1|] eqn:Hcorq1; simpl in *; [|auto].
-          destruct (orqs@[child2Idx]) as [corq2|] eqn:Hcorq2; simpl in *; [|auto].
-          destruct H6 as [[cv ?] ?].
-          red in H6; dest.
-          split.
-          * exists cv.
-            clear H8.
-            red; repeat ssplit.
-            { solve_rule_conds_ex.
-              right; left.
-              destruct H6 as [|[|]].
-              { solve_rule_conds_ex; solve_msi. }
+        + apply Forall_app.
+          * apply forall_removeOnce.
+            eapply atomic_rqUp_preserves_msg_out_preds with (oidx:= child2Idx);
+              [exact msiSv_impl_ORqsInit
+              |exact msiSv_impl_RqRsSys|..]; eauto.
+            { intro; dest_in; discriminate. }
+            { red; auto. }
+            { exact msiSvMsgOutPred_good. }
+          * repeat (constructor; simpl).
+            red; repeat (simpl; mred).
+        + destruct H6; split.
+          * red in H6; red; simpl in *; mred; simpl.
+            destruct (oss@[child1Idx]) as [cost1|] eqn:Hcost1; simpl in *; [|auto].
+            destruct (oss@[child2Idx]) as [cost2|] eqn:Hcost2; simpl in *; [|auto].
+            destruct (orqs@[child1Idx]) as [corq1|] eqn:Hcorq1; simpl in *; [|auto].
+            destruct (orqs@[child2Idx]) as [corq2|] eqn:Hcorq2; simpl in *; [|auto].
+            destruct H6 as [[cv ?] ?].
+            red in H6; dest.
+            split.
+            { exists cv.
+              red; repeat ssplit.
+              { solve_rule_conds_ex.
+                right; left.
+                destruct H6 as [|[|]].
+                { solve_rule_conds_ex; solve_msi. }
+                { solve_rule_conds_ex. }
+                { solve_msi. }
+              }
               { solve_rule_conds_ex. }
-              { solve_msi. }
+              { solve_rule_conds_ex. }
+              { solve_rule_conds_ex. }
             }
-            { solve_rule_conds_ex. }
-            { solve_rule_conds_ex. }
-            { solve_rule_conds_ex. }
-          * disc_rule_conds_ex.
-            assert (In (child child2Idx ec2 ce2 c2pRq c2pRs pc2) (sys_objs impl))
-              by (simpl; tauto).
-            good_locking_get (child child2Idx ec2 ce2 c2pRq c2pRs pc2).
-            clear H24.
-            eapply upLockInvORq_rqUp_length_one_locked in H26; try reflexivity;
-              [|eapply findQ_length_ge_one; apply FirstMP_InMP; eassumption].
-            solve_rule_conds_ex.
+            { disc_rule_conds_ex.
+              assert (In (child child2Idx ec2 ce2 c2pRq c2pRs pc2) (sys_objs impl))
+                by (simpl; tauto).
+              good_locking_get (child child2Idx ec2 ce2 c2pRq c2pRs pc2).
+              clear H24.
+              eapply upLockInvORq_rqUp_length_one_locked in H26; try reflexivity;
+                [|eapply findQ_length_ge_one; apply FirstMP_InMP; eassumption].
+              solve_rule_conds_ex.
+            }
+          * red in H7; red; simpl in *; mred.
 
       - (** [parentGetDownRqS] *)
         disc_rule_conds_ex.
 
         split.
-        + split.
-          * apply Forall_app.
-            { apply forall_removeOnce.
-              eapply atomic_rqUp_preserves_msg_out_preds with (oidx:= child2Idx);
-                [exact msiSv_impl_ORqsInit
-                |exact msiSv_impl_RqRsSys|..]; eauto.
-              { intro; dest_in; discriminate. }
-              { red; auto. }
-              { exact msiSvMsgOutPred_good. }
-            }
-            { repeat (constructor; simpl). }
-          * red; simpl; intros.
-            icase oidx.
-            { repeat (simpl; red; mred).
-              simpl; right; auto.
-            }
-            { mred; apply H7; auto. }
-        + red in H6; red; simpl in *; mred.
+        + apply Forall_app.
+          * apply forall_removeOnce.
+            eapply atomic_rqUp_preserves_msg_out_preds with (oidx:= child2Idx);
+              [exact msiSv_impl_ORqsInit
+              |exact msiSv_impl_RqRsSys|..]; eauto.
+            { intro; dest_in; discriminate. }
+            { red; auto. }
+            { exact msiSvMsgOutPred_good. }
+          * repeat (constructor; simpl).
+        + destruct H6; split.
+          * red in H6; red; simpl in *; mred.
+          * solve_rule_conds_ex.
 
       - (** [parentSetRqImm] *)
         disc_rule_conds_ex.
 
         split.
-        + split.
-          * apply Forall_app.
-            { apply forall_removeOnce.
-              eapply atomic_rqUp_preserves_msg_out_preds with (oidx:= child2Idx);
-                [exact msiSv_impl_ORqsInit
-                |exact msiSv_impl_RqRsSys|..]; eauto.
-              { intro; dest_in; discriminate. }
-              { red; auto. }
-              { exact msiSvMsgOutPred_good. }
+        + apply Forall_app.
+          * apply forall_removeOnce.
+            eapply atomic_rqUp_preserves_msg_out_preds with (oidx:= child2Idx);
+              [exact msiSv_impl_ORqsInit
+              |exact msiSv_impl_RqRsSys|..]; eauto.
+            { intro; dest_in; discriminate. }
+            { red; auto. }
+            { exact msiSvMsgOutPred_good. }
+          * repeat (constructor; simpl).
+            red; repeat (simpl; mred).
+        + destruct H6; split.
+          * red in H6; red; simpl in *; mred; simpl.
+            destruct (oss@[child1Idx]) as [cost1|] eqn:Hcost1; simpl in *; [|auto].
+            destruct (oss@[child2Idx]) as [cost2|] eqn:Hcost2; simpl in *; [|auto].
+            destruct (orqs@[child1Idx]) as [corq1|] eqn:Hcorq1; simpl in *; [|auto].
+            destruct (orqs@[child2Idx]) as [corq2|] eqn:Hcorq2; simpl in *; [|auto].
+            destruct H6 as [[cv ?] ?].
+            red in H6; dest.
+            unfold getDir in H14; simpl in H14.
+            split.
+            { exists cv.
+              red; repeat ssplit.
+              { solve_rule_conds_ex.
+                right; right; auto.
+              }
+              { solve_rule_conds_ex. }
+              { solve_rule_conds_ex. }
+              { solve_rule_conds_ex. }
             }
-            { repeat (constructor; simpl).
-              red; repeat (simpl; mred).
+            { disc_rule_conds_ex.
+              assert (In (child child2Idx ec2 ce2 c2pRq c2pRs pc2) (sys_objs impl))
+                by (simpl; tauto).
+              good_locking_get (child child2Idx ec2 ce2 c2pRq c2pRs pc2).
+              clear H24.
+              eapply upLockInvORq_rqUp_length_one_locked in H26; try reflexivity;
+                [|eapply findQ_length_ge_one; apply FirstMP_InMP; eassumption].
+              solve_rule_conds_ex.
             }
-          * red; simpl; intros.
-            icase oidx.
-            { repeat (simpl; red; mred). }
-            { mred; apply H7; auto. }
-        + red in H6; red; simpl in *; mred; simpl.
-          destruct (oss@[child1Idx]) as [cost1|] eqn:Hcost1; simpl in *; [|auto].
-          destruct (oss@[child2Idx]) as [cost2|] eqn:Hcost2; simpl in *; [|auto].
-          destruct (orqs@[child1Idx]) as [corq1|] eqn:Hcorq1; simpl in *; [|auto].
-          destruct (orqs@[child2Idx]) as [corq2|] eqn:Hcorq2; simpl in *; [|auto].
-          destruct H6 as [[cv ?] ?].
-          red in H6; dest.
-          unfold getDir in H14; simpl in H14.
-          split.
-          * exists cv.
-            red; repeat ssplit.
-            { solve_rule_conds_ex.
-              right; right; auto.
-            }
-            { solve_rule_conds_ex. }
-            { solve_rule_conds_ex. }
-            { solve_rule_conds_ex. }
-          * disc_rule_conds_ex.
-            assert (In (child child2Idx ec2 ce2 c2pRq c2pRs pc2) (sys_objs impl))
-              by (simpl; tauto).
-            good_locking_get (child child2Idx ec2 ce2 c2pRq c2pRs pc2).
-            clear H24.
-            eapply upLockInvORq_rqUp_length_one_locked in H26; try reflexivity;
-              [|eapply findQ_length_ge_one; apply FirstMP_InMP; eassumption].
-            solve_rule_conds_ex.
+          * red in H7; red; simpl in *; mred.
 
       - (** [parentSetDownRqM] *)
         disc_rule_conds_ex.
 
         split.
-        + split.
-          * apply Forall_app.
-            { apply forall_removeOnce.
-              eapply atomic_rqUp_preserves_msg_out_preds with (oidx:= child2Idx);
-                [exact msiSv_impl_ORqsInit
-                |exact msiSv_impl_RqRsSys|..]; eauto.
-              { intro; dest_in; discriminate. }
-              { red; auto. }
-              { exact msiSvMsgOutPred_good. }
-            }
-            { repeat (constructor; simpl). }
-          * red; simpl; intros.
-            icase oidx.
-            { repeat (simpl; red; mred).
-              simpl; right; auto.
-            }
-            { mred; apply H7; auto. }
-        + red in H6; red; simpl in *; mred.
+        + apply Forall_app.
+          * apply forall_removeOnce.
+            eapply atomic_rqUp_preserves_msg_out_preds with (oidx:= child2Idx);
+              [exact msiSv_impl_ORqsInit
+              |exact msiSv_impl_RqRsSys|..]; eauto.
+            { intro; dest_in; discriminate. }
+            { red; auto. }
+            { exact msiSvMsgOutPred_good. }
+          * repeat (constructor; simpl).
+        + destruct H6; split.
+          * red in H6; red; simpl in *; mred.
+          * solve_rule_conds_ex.
 
       - (** [parentGetDownRsS] *)
         disc_rule_conds_ex.
 
-        obj_visited_rsUp parentIdx child1Idx.
-        disc_lock_preds parentIdx.
-        disc_rule_conds_ex.
-        destruct H11; dest; [discriminate|].
-        clear H11.
-        disc_rule_conds_ex.
+        (* discharge the lock invariant *)
+        destruct H6.
+        red in H8; simpl in H8.
+        disc_rule_conds_const.
+        red in H8.
+        disc_rule_conds_const.
+        destruct H8; dest; [discriminate|].
+        rewrite H10 in *.
 
         (* discharge message predicates *)
         disc_msg_preds H4.
         disc_rule_conds_ex.
         
         split.
-        + split.
-          * apply Forall_app.
-            { apply forall_removeOnce.
-              eapply atomic_rsUps_preserves_msg_out_preds
-                with (rsUps:= [(c1pRs, rmsg)]); eauto.
-              { exact msiSv_impl_ORqsInit. }
-              { exact msiSv_impl_RqRsSys. }
-              { repeat constructor; intro; dest_in. }
-              { apply SubList_cons; [|apply SubList_nil].
-                assumption.
-              }
-              { instantiate (1:= fun _ => True).
-                instantiate (1:= [pc1]).
+        + apply Forall_app.
+          * apply forall_removeOnce.
+            eapply atomic_rsUps_preserves_msg_out_preds
+              with (rsUps:= [(c1pRs, rmsg)]); eauto.
+            { exact msiSv_impl_ORqsInit. }
+            { exact msiSv_impl_RqRsSys. }
+            { repeat constructor; intro; dest_in. }
+            { apply SubList_cons; [|apply SubList_nil].
+              assumption.
+            }
+            { instantiate (1:= fun _ => True).
+              instantiate (1:= [pc1]).
+              repeat split.
+              { discriminate. }
+              { repeat constructor.
+                simpl; exists child1Idx.
                 repeat split.
-                { discriminate. }
-                { repeat constructor.
-                  simpl; exists child1Idx.
-                  repeat split.
-                }
               }
-              { exact msiSvMsgOutPred_good. }
             }
-            { repeat (constructor; simpl).
-              red; simpl.
-              solve_rule_conds_ex.
-            }
-          * red; simpl; intros.
-            icase oidx.
-            { repeat (simpl; red; mred). }
-            { mred; apply H7; auto. }
-        + red in H6; red; simpl in *; mred; simpl.
-          destruct (oss@[child2Idx]) as [cost2|] eqn:Hcost2; simpl in *; [|auto].
-          destruct (orqs@[child1Idx]) as [corq1|] eqn:Hcorq1; simpl in *; [|auto].
-          destruct (orqs@[child2Idx]) as [corq2|] eqn:Hcorq2; simpl in *; [|auto].
-          destruct H6 as [[cv ?] ?].
-          red in H6; dest.
+            { exact msiSvMsgOutPred_good. }
+          * repeat (constructor; simpl).
+            red; simpl.
+            solve_rule_conds_ex.
+        + split.
+          * red in H6; red; simpl in *; mred; simpl.
+            destruct (oss@[child2Idx]) as [cost2|] eqn:Hcost2; simpl in *; [|auto].
+            destruct (orqs@[child1Idx]) as [corq1|] eqn:Hcorq1; simpl in *; [|auto].
+            destruct (orqs@[child2Idx]) as [corq2|] eqn:Hcorq2; simpl in *; [|auto].
+            destruct H6 as [[cv ?] ?].
+            red in H6; dest.
 
-          assert (In (child child2Idx ec2 ce2 c2pRq c2pRs pc2) (sys_objs impl))
-            by (simpl; tauto).
-          good_locking_get (child child2Idx ec2 ce2 c2pRq c2pRs pc2).
-          clear H24.
-          eapply upLockInvORq_parent_locked_locked in H26; try reflexivity;
-            [|red; repeat (simpl; mred); eauto]; dest.
+            assert (In (child child2Idx ec2 ce2 c2pRq c2pRs pc2) (sys_objs impl))
+              by (simpl; tauto).
+            good_locking_get (child child2Idx ec2 ce2 c2pRq c2pRs pc2).
+            clear H21.
+            eapply upLockInvORq_parent_locked_locked in H22; try reflexivity;
+              [|red; repeat (simpl; mred); eauto]; dest.
           
-          split.
-          * exists val0.
-            clear H11.
-            red; repeat ssplit.
-            { solve_rule_conds_ex.
-              right; left; auto.
+            split.
+            { exists val0.
+              red; repeat ssplit.
+              { solve_rule_conds_ex.
+                right; left; auto.
+              }
+              { solve_rule_conds_ex. }
+              { solve_rule_conds_ex. }
+              { solve_rule_conds_ex. }
             }
-            { solve_rule_conds_ex. }
-            { solve_rule_conds_ex. }
             { solve_rule_conds_ex. }
           * solve_rule_conds_ex.
 
       - (** [parentSetDownRsM] *)
         disc_rule_conds_ex.
 
-        obj_visited_rsUp parentIdx child1Idx.
-        disc_lock_preds parentIdx.
-        disc_rule_conds_ex.
-        destruct H11; dest; [discriminate|].
-        clear H11.
-        disc_rule_conds_ex.
+        (* discharge the lock invariant *)
+        destruct H6.
+        red in H8; simpl in H8.
+        disc_rule_conds_const.
+        red in H8.
+        disc_rule_conds_const.
+        destruct H8; dest; [discriminate|].
+        rewrite H10 in *.
 
         (* discharge message predicates *)
         disc_msg_preds H4.
         disc_rule_conds_ex.
         
         split.
-        + split.
-          * apply Forall_app.
-            { apply forall_removeOnce.
-              eapply atomic_rsUps_preserves_msg_out_preds
-                with (rsUps:= [(c1pRs, rmsg)]); eauto.
-              { exact msiSv_impl_ORqsInit. }
-              { exact msiSv_impl_RqRsSys. }
-              { repeat constructor; intro; dest_in. }
-              { apply SubList_cons; [|apply SubList_nil].
-                assumption.
-              }
-              { instantiate (1:= fun _ => True).
-                instantiate (1:= [pc1]).
+        + apply Forall_app.
+          * apply forall_removeOnce.
+            eapply atomic_rsUps_preserves_msg_out_preds
+              with (rsUps:= [(c1pRs, rmsg)]); eauto.
+            { exact msiSv_impl_ORqsInit. }
+            { exact msiSv_impl_RqRsSys. }
+            { repeat constructor; intro; dest_in. }
+            { apply SubList_cons; [|apply SubList_nil].
+              assumption.
+            }
+            { instantiate (1:= fun _ => True).
+              instantiate (1:= [pc1]).
+              repeat split.
+              { discriminate. }
+              { repeat constructor.
+                simpl; exists child1Idx.
                 repeat split.
-                { discriminate. }
-                { repeat constructor.
-                  simpl; exists child1Idx.
-                  repeat split.
-                }
               }
-              { exact msiSvMsgOutPred_good. }
             }
-            { repeat (constructor; simpl).
-              red; simpl.
-              solve_rule_conds_ex.
-            }
-          * red; simpl; intros.
-            icase oidx.
-            { repeat (simpl; red; mred). }
-            { mred; apply H7; auto. }
-        + red in H6; red; simpl in *; mred; simpl.
-          destruct (oss@[child2Idx]) as [cost2|] eqn:Hcost1; simpl in *; [|auto].
-          destruct (orqs@[child1Idx]) as [corq1|] eqn:Hcorq1; simpl in *; [|auto].
-          destruct (orqs@[child2Idx]) as [corq2|] eqn:Hcorq2; simpl in *; [|auto].
-          destruct H6 as [[cv ?] ?].
-          red in H6; dest.
+            { exact msiSvMsgOutPred_good. }
+          * repeat (constructor; simpl).
+            red; simpl.
+            solve_rule_conds_ex.
+        + split.
+          * red in H6; red; simpl in *; mred; simpl.
+            destruct (oss@[child2Idx]) as [cost2|] eqn:Hcost2; simpl in *; [|auto].
+            destruct (orqs@[child1Idx]) as [corq1|] eqn:Hcorq1; simpl in *; [|auto].
+            destruct (orqs@[child2Idx]) as [corq2|] eqn:Hcorq2; simpl in *; [|auto].
+            destruct H6 as [[cv ?] ?].
+            red in H6; dest.
 
-          assert (In (child child2Idx ec2 ce2 c2pRq c2pRs pc2) (sys_objs impl))
-            by (simpl; tauto).
-          good_locking_get (child child2Idx ec2 ce2 c2pRq c2pRs pc2).
-          clear H24.
-          eapply upLockInvORq_parent_locked_locked in H26; try reflexivity;
-            [|red; repeat (simpl; mred); eauto]; dest.
+            assert (In (child child2Idx ec2 ce2 c2pRq c2pRs pc2) (sys_objs impl))
+              by (simpl; tauto).
+            good_locking_get (child child2Idx ec2 ce2 c2pRq c2pRs pc2).
+            clear H21.
+            eapply upLockInvORq_parent_locked_locked in H22; try reflexivity;
+              [|red; repeat (simpl; mred); eauto]; dest.
 
-          split.
-          * exists val0.
-            clear H11.
-            red; repeat ssplit.
-            { solve_rule_conds_ex.
-              right; right; auto.
+            split.
+            { exists val0.
+              red; repeat ssplit.
+              { solve_rule_conds_ex.
+                right; right; auto.
+              }
+              { solve_rule_conds_ex. }
+              { solve_rule_conds_ex. }
+              { solve_rule_conds_ex. }
             }
-            { solve_rule_conds_ex. }
-            { solve_rule_conds_ex. }
             { solve_rule_conds_ex. }
           * solve_rule_conds_ex.
 
@@ -1803,182 +1771,167 @@ Section Inv.
         disc_rule_conds_ex.
 
         split.
-        + split.
-          * apply Forall_app.
-            { apply forall_removeOnce.
-              eapply atomic_rqUp_preserves_msg_out_preds with (oidx:= child2Idx);
-                [exact msiSv_impl_ORqsInit
-                |exact msiSv_impl_RqRsSys|..]; eauto.
-              { intro; dest_in; discriminate. }
-              { red; auto. }
-              { exact msiSvMsgOutPred_good. }
-            }
-            { repeat (constructor; simpl).
-              red; repeat (simpl; mred).
-            }
-          * red; simpl; intros.
-            icase oidx.
-            { repeat (simpl; red; mred). }
-            { mred; apply H7; auto. }
-        + red in H6; red; simpl in *; mred.
-            
+        + apply Forall_app.
+          * apply forall_removeOnce.
+            eapply atomic_rqUp_preserves_msg_out_preds with (oidx:= child2Idx);
+              [exact msiSv_impl_ORqsInit
+              |exact msiSv_impl_RqRsSys|..]; eauto.
+            { intro; dest_in; discriminate. }
+            { red; auto. }
+            { exact msiSvMsgOutPred_good. }
+          * repeat (constructor; simpl).
+            red; repeat (simpl; mred).
+        + destruct H6; split.
+          * red in H6; red; simpl in *; mred.
+          * red in H7; red; simpl in *; mred.
+        
       - (** [parentEvictRqImmS] *)
         disc_rule_conds_ex.
 
         split.
-        + split.
-          * apply Forall_app.
-            { apply forall_removeOnce.
-              eapply atomic_rqUp_preserves_msg_out_preds with (oidx:= child2Idx);
-                [exact msiSv_impl_ORqsInit
-                |exact msiSv_impl_RqRsSys|..]; eauto.
-              { intro; dest_in; discriminate. }
-              { red; auto. }
-              { exact msiSvMsgOutPred_good. }
+        + apply Forall_app.
+          * apply forall_removeOnce.
+            eapply atomic_rqUp_preserves_msg_out_preds with (oidx:= child2Idx);
+              [exact msiSv_impl_ORqsInit
+              |exact msiSv_impl_RqRsSys|..]; eauto.
+            { intro; dest_in; discriminate. }
+            { red; auto. }
+            { exact msiSvMsgOutPred_good. }
+          * repeat (constructor; simpl).
+            red; repeat (simpl; mred).
+        + destruct H6; split.
+          * red in H6; red; simpl in *; mred; simpl.
+            destruct (oss@[child1Idx]) as [cost1|] eqn:Hcost1; simpl in *; [|auto].
+            destruct (oss@[child2Idx]) as [cost2|] eqn:Hcost2; simpl in *; [|auto].
+            destruct (orqs@[child1Idx]) as [corq1|] eqn:Hcorq1; simpl in *; [|auto].
+            destruct (orqs@[child2Idx]) as [corq2|] eqn:Hcorq2; simpl in *; [|auto].
+            destruct H6 as [[cv ?] ?].
+            red in H6; dest.
+            unfold getDir in *; simpl in *.
+            disc_rule_conds_ex.
+            destruct H6 as [|[|]];
+              [exfalso; solve_rule_conds_ex
+              | |exfalso; destruct H6 as [? [|]]; solve_rule_conds_ex].
+            split.
+            { exists cv.
+              repeat ssplit.
+              { solve_rule_conds_ex.
+                right; left; solve_msi.
+              }
+              { solve_rule_conds_ex. }
+              { solve_rule_conds_ex. }
+              { solve_rule_conds_ex. }
             }
-            { repeat (constructor; simpl).
-              red; repeat (simpl; mred).
+            { disc_rule_conds_ex.
+              assert (In (child child2Idx ec2 ce2 c2pRq c2pRs pc2) (sys_objs impl))
+                by (simpl; tauto).
+              good_locking_get (child child2Idx ec2 ce2 c2pRq c2pRs pc2).
+              clear H6.
+              eapply upLockInvORq_rqUp_length_one_locked in H28; try reflexivity;
+                [|eapply findQ_length_ge_one; apply FirstMP_InMP; eassumption].
+              solve_rule_conds_ex.
             }
-          * red; simpl; intros.
-            icase oidx.
-            { repeat (simpl; red; mred). }
-            { mred; apply H7; auto. }
-        + red in H6; red; simpl in *; mred; simpl.
-          destruct (oss@[child1Idx]) as [cost1|] eqn:Hcost1; simpl in *; [|auto].
-          destruct (oss@[child2Idx]) as [cost2|] eqn:Hcost2; simpl in *; [|auto].
-          destruct (orqs@[child1Idx]) as [corq1|] eqn:Hcorq1; simpl in *; [|auto].
-          destruct (orqs@[child2Idx]) as [corq2|] eqn:Hcorq2; simpl in *; [|auto].
-          destruct H6 as [[cv ?] ?].
-          red in H6; dest.
-          unfold getDir in *; simpl in *.
-          disc_rule_conds_ex.
-          destruct H6 as [|[|]];
-            [exfalso; solve_rule_conds_ex
-            | |exfalso; destruct H6 as [? [|]]; solve_rule_conds_ex].
-          split.
-          * exists cv.
-            repeat ssplit.
-            { solve_rule_conds_ex.
-              right; left; solve_msi.
-            }
-            { solve_rule_conds_ex. }
-            { solve_rule_conds_ex. }
-            { solve_rule_conds_ex. }
-          * disc_rule_conds_ex.
-            assert (In (child child2Idx ec2 ce2 c2pRq c2pRs pc2) (sys_objs impl))
-              by (simpl; tauto).
-            good_locking_get (child child2Idx ec2 ce2 c2pRq c2pRs pc2).
-            clear H6.
-            eapply upLockInvORq_rqUp_length_one_locked in H28; try reflexivity;
-              [|eapply findQ_length_ge_one; apply FirstMP_InMP; eassumption].
-            solve_rule_conds_ex.
+          * red in H7; red; simpl in *; mred.
 
       - (** [parentEvictRqImmLastS] *)
         disc_rule_conds_ex.
 
         split.
-        + split.
-          * apply Forall_app.
-            { apply forall_removeOnce.
-              eapply atomic_rqUp_preserves_msg_out_preds with (oidx:= child2Idx);
-                [exact msiSv_impl_ORqsInit
-                |exact msiSv_impl_RqRsSys|..]; eauto.
-              { intro; dest_in; discriminate. }
-              { red; auto. }
-              { exact msiSvMsgOutPred_good. }
+        + apply Forall_app.
+          * apply forall_removeOnce.
+            eapply atomic_rqUp_preserves_msg_out_preds with (oidx:= child2Idx);
+              [exact msiSv_impl_ORqsInit
+              |exact msiSv_impl_RqRsSys|..]; eauto.
+            { intro; dest_in; discriminate. }
+            { red; auto. }
+            { exact msiSvMsgOutPred_good. }
+          * repeat (constructor; simpl).
+            red; repeat (simpl; mred).
+        + destruct H6; split.
+          * red in H6; red; simpl in *; mred; simpl.
+            destruct (oss@[child1Idx]) as [cost1|] eqn:Hcost1; simpl in *; [|auto].
+            destruct (oss@[child2Idx]) as [cost2|] eqn:Hcost2; simpl in *; [|auto].
+            destruct (orqs@[child1Idx]) as [corq1|] eqn:Hcorq1; simpl in *; [|auto].
+            destruct (orqs@[child2Idx]) as [corq2|] eqn:Hcorq2; simpl in *; [|auto].
+            destruct H6 as [[cv ?] ?].
+            red in H6; dest.
+            unfold getDir in *; simpl in *.
+            disc_rule_conds_ex.
+            destruct H6 as [|[|]];
+              [exfalso; solve_rule_conds_ex
+              | |exfalso; destruct H6 as [? [|]]; solve_rule_conds_ex].
+            split.
+            { exists cv.
+              repeat ssplit.
+              { solve_rule_conds_ex.
+                left; auto.
+              }
+              { solve_rule_conds_ex. }
+              { solve_rule_conds_ex. }
+              { solve_rule_conds_ex. }
             }
-            { repeat (constructor; simpl).
-              red; repeat (simpl; mred).
+            { disc_rule_conds_ex.
+              assert (In (child child2Idx ec2 ce2 c2pRq c2pRs pc2) (sys_objs impl))
+                by (simpl; tauto).
+              good_locking_get (child child2Idx ec2 ce2 c2pRq c2pRs pc2).
+              clear H6.
+              eapply upLockInvORq_rqUp_length_one_locked in H28; try reflexivity;
+                [|eapply findQ_length_ge_one; apply FirstMP_InMP; eassumption].
+              solve_rule_conds_ex.
             }
-          * red; simpl; intros.
-            icase oidx.
-            { repeat (simpl; red; mred). }
-            { mred; apply H7; auto. }
-        + red in H6; red; simpl in *; mred; simpl.
-          destruct (oss@[child1Idx]) as [cost1|] eqn:Hcost1; simpl in *; [|auto].
-          destruct (oss@[child2Idx]) as [cost2|] eqn:Hcost2; simpl in *; [|auto].
-          destruct (orqs@[child1Idx]) as [corq1|] eqn:Hcorq1; simpl in *; [|auto].
-          destruct (orqs@[child2Idx]) as [corq2|] eqn:Hcorq2; simpl in *; [|auto].
-          destruct H6 as [[cv ?] ?].
-          red in H6; dest.
-          unfold getDir in *; simpl in *.
-          disc_rule_conds_ex.
-          destruct H6 as [|[|]];
-            [exfalso; solve_rule_conds_ex
-            | |exfalso; destruct H6 as [? [|]]; solve_rule_conds_ex].
-          split.
-          * exists cv.
-            repeat ssplit.
-            { solve_rule_conds_ex.
-              left; auto.
-            }
-            { solve_rule_conds_ex. }
-            { solve_rule_conds_ex. }
-            { solve_rule_conds_ex. }
-          * disc_rule_conds_ex.
-            assert (In (child child2Idx ec2 ce2 c2pRq c2pRs pc2) (sys_objs impl))
-              by (simpl; tauto).
-            good_locking_get (child child2Idx ec2 ce2 c2pRq c2pRs pc2).
-            clear H6.
-            eapply upLockInvORq_rqUp_length_one_locked in H28; try reflexivity;
-              [|eapply findQ_length_ge_one; apply FirstMP_InMP; eassumption].
-            solve_rule_conds_ex.
+          * red in H7; red; simpl in *; mred.
 
       - (** [parentEvictRqImmM] *)
         disc_rule_conds_ex.
 
         split.
-        + split.
-          * apply Forall_app.
-            { apply forall_removeOnce.
-              eapply atomic_rqUp_preserves_msg_out_preds with (oidx:= child2Idx);
-                [exact msiSv_impl_ORqsInit
-                |exact msiSv_impl_RqRsSys|..]; eauto.
-              { intro; dest_in; discriminate. }
-              { red; auto. }
-              { exact msiSvMsgOutPred_good. }
-            }
-            { repeat (constructor; simpl).
-              red; repeat (simpl; mred).
-            }
-          * red; simpl; intros.
-            icase oidx.
-            { repeat (simpl; red; mred). }
-            { mred; apply H7; auto. }
-        + red in H6; red; simpl in *; mred; simpl.
-          destruct (oss@[child1Idx]) as [cost1|] eqn:Hcost1; simpl in *; [|auto].
-          destruct (oss@[child2Idx]) as [cost2|] eqn:Hcost2; simpl in *; [|auto].
-          destruct (orqs@[child1Idx]) as [corq1|] eqn:Hcorq1; simpl in *; [|auto].
-          destruct (orqs@[child2Idx]) as [corq2|] eqn:Hcorq2; simpl in *; [|auto].
-          destruct H6 as [[cv ?] ?].
-          red in H6; dest.
-          unfold getDir in *; simpl in *.
-          disc_rule_conds_ex.
-          destruct H6 as [|[|]]; try (exfalso; solve_rule_conds_ex; fail).
+        + apply Forall_app.
+          * apply forall_removeOnce.
+            eapply atomic_rqUp_preserves_msg_out_preds with (oidx:= child2Idx);
+              [exact msiSv_impl_ORqsInit
+              |exact msiSv_impl_RqRsSys|..]; eauto.
+            { intro; dest_in; discriminate. }
+            { red; auto. }
+            { exact msiSvMsgOutPred_good. }
+          * repeat (constructor; simpl).
+            red; repeat (simpl; mred).
+        + destruct H6; split.
+          * red in H6; red; simpl in *; mred; simpl.
+            destruct (oss@[child1Idx]) as [cost1|] eqn:Hcost1; simpl in *; [|auto].
+            destruct (oss@[child2Idx]) as [cost2|] eqn:Hcost2; simpl in *; [|auto].
+            destruct (orqs@[child1Idx]) as [corq1|] eqn:Hcorq1; simpl in *; [|auto].
+            destruct (orqs@[child2Idx]) as [corq2|] eqn:Hcorq2; simpl in *; [|auto].
+            destruct H6 as [[cv ?] ?].
+            red in H6; dest.
+            unfold getDir in *; simpl in *.
+            disc_rule_conds_ex.
+            destruct H6 as [|[|]]; try (exfalso; solve_rule_conds_ex; fail).
 
-          assert (In (child child2Idx ec2 ce2 c2pRq c2pRs pc2) (sys_objs impl))
-            by (simpl; tauto).
-          good_locking_get (child child2Idx ec2 ce2 c2pRq c2pRs pc2).
-          clear H26.
-          eapply upLockInvORq_rqUp_length_one_locked in H27; try reflexivity;
-            [|eapply findQ_length_ge_one; apply FirstMP_InMP; eassumption].
-          disc_rule_conds_ex.
+            assert (In (child child2Idx ec2 ce2 c2pRq c2pRs pc2) (sys_objs impl))
+              by (simpl; tauto).
+            good_locking_get (child child2Idx ec2 ce2 c2pRq c2pRs pc2).
+            clear H26.
+            eapply upLockInvORq_rqUp_length_one_locked in H27; try reflexivity;
+              [|eapply findQ_length_ge_one; apply FirstMP_InMP; eassumption].
+            disc_rule_conds_ex.
           
-          split.
-          * exists n.
-            repeat ssplit.
-            { solve_rule_conds_ex.
-              left; solve_msi.
+            split.
+            { exists n.
+              repeat ssplit.
+              { solve_rule_conds_ex.
+                left; solve_msi.
+              }
+              { solve_rule_conds_ex; solve_msi. }
+              { solve_rule_conds_ex. }
+              { solve_rule_conds_ex. }
             }
-            { solve_rule_conds_ex; solve_msi. }
             { solve_rule_conds_ex. }
-            { solve_rule_conds_ex. }
-          * solve_rule_conds_ex.
+          * red in H7; red; simpl in *; mred.
 
     Qed.
 
-    Lemma ImplStateInv_init:
-      ImplStateInv (initsOf impl).
+    Lemma implInv_init:
+      ImplInv (initsOf impl).
     Proof.
       red; simpl.
       unfold implOStatesInit, implORqsInit; mred.
@@ -1994,11 +1947,11 @@ Section Inv.
       - vm_compute; intros; auto.
     Qed.
 
-    Lemma ImplStateInv_invStep:
-      InvStep impl step_m ImplStateInv.
+    Lemma implInv_invStep:
+      InvStep impl step_m ImplInv.
     Proof.
       apply invSeq_serializable_invStep.
-      - apply ImplStateInv_init.
+      - apply implInv_init.
       - apply inv_trs_seqSteps.
         apply msiSv_impl_InvTrs.
       - eapply rqrs_Serializable.
